more

Weidenbach_Book/Watched_Literals_VMTF.thy
@@ -979,9 +979,6 @@ next
 qed
 
 
-context isasat_input_bounded_nempty
-begin
-
 paragraph \<open>Abstract Invariants\<close>
 
 text \<open>
@@ -992,16 +989,16 @@ text \<open>
   \<^item> The atoms of \<^term>\<open>zs\<close> are either in \<^term>\<open>xs\<close> and \<^term>\<open>ys\<close>.
 \<close>
 
-definition (in isasat_input_ops) vmtf_\<L>\<^sub>a\<^sub>l\<^sub>l :: \<open>(nat, nat) ann_lits \<Rightarrow> nat abs_vmtf_ns_remove \<Rightarrow> bool\<close> where
-\<open>vmtf_\<L>\<^sub>a\<^sub>l\<^sub>l M \<equiv> \<lambda>((xs, ys), zs).
+definition vmtf_\<L>\<^sub>a\<^sub>l\<^sub>l :: \<open>nat multiset \<Rightarrow> (nat, nat) ann_lits \<Rightarrow> nat abs_vmtf_ns_remove \<Rightarrow> bool\<close> where
+\<open>vmtf_\<L>\<^sub>a\<^sub>l\<^sub>l \<A> M \<equiv> \<lambda>((xs, ys), zs).
   (\<forall>L\<in>ys. L \<in> atm_of ` lits_of_l M) \<and>
   xs \<inter> ys = {} \<and>
   zs \<subseteq> xs \<union> ys \<and>
-  xs \<union> ys = atms_of \<L>\<^sub>a\<^sub>l\<^sub>l
+  xs \<union> ys = atms_of (\<L>\<^sub>a\<^sub>l\<^sub>l \<A>)
   \<close>
 
-abbreviation abs_vmtf_ns_inv :: \<open>(nat, nat) ann_lits \<Rightarrow> nat abs_vmtf_ns \<Rightarrow> bool\<close> where
-\<open>abs_vmtf_ns_inv M vm \<equiv> vmtf_\<L>\<^sub>a\<^sub>l\<^sub>l M (vm, {})\<close>
+abbreviation abs_vmtf_ns_inv :: \<open>nat multiset \<Rightarrow> (nat, nat) ann_lits \<Rightarrow> nat abs_vmtf_ns \<Rightarrow> bool\<close> where
+\<open>abs_vmtf_ns_inv \<A> M vm \<equiv> vmtf_\<L>\<^sub>a\<^sub>l\<^sub>l \<A> M (vm, {})\<close>
 
 
 subsubsection \<open>Implementation\<close>
@@ -1014,39 +1011,39 @@ text \<open>
   the beginning.
 \<close>
 
-definition (in isasat_input_ops) vmtf :: \<open>(nat, nat) ann_lits \<Rightarrow> vmtf_remove_int set\<close> where
-\<open>vmtf M = {((ns, m, fst_As, lst_As, next_search), to_remove).
+definition vmtf :: \<open>nat multiset \<Rightarrow> (nat, nat) ann_lits \<Rightarrow> vmtf_remove_int set\<close> where
+\<open>vmtf \<A> M = {((ns, m, fst_As, lst_As, next_search), to_remove).
    (\<exists>xs' ys'.
      vmtf_ns (ys' @ xs') m ns \<and> fst_As = hd (ys' @ xs') \<and> lst_As = last (ys' @ xs')
    \<and> next_search = option_hd xs'
-   \<and> vmtf_\<L>\<^sub>a\<^sub>l\<^sub>l M ((set xs', set ys'), to_remove)
+   \<and> vmtf_\<L>\<^sub>a\<^sub>l\<^sub>l \<A> M ((set xs', set ys'), to_remove)
    \<and> vmtf_ns_notin (ys' @ xs') m ns
-   \<and> (\<forall>L\<in>atms_of \<L>\<^sub>a\<^sub>l\<^sub>l. L < length ns) \<and> (\<forall>L\<in>set (ys' @ xs'). L \<in> atms_of \<L>\<^sub>a\<^sub>l\<^sub>l)
+   \<and> (\<forall>L\<in>atms_of (\<L>\<^sub>a\<^sub>l\<^sub>l \<A>). L < length ns) \<and> (\<forall>L\<in>set (ys' @ xs'). L \<in> atms_of (\<L>\<^sub>a\<^sub>l\<^sub>l \<A>))
   )}\<close>
 
-lemma (in isasat_input_ops) vmtf_consD:
-  assumes vmtf: \<open>((ns, m, fst_As, lst_As, next_search), remove) \<in> vmtf M\<close>
-  shows \<open>((ns, m, fst_As, lst_As, next_search), remove) \<in> vmtf (L # M)\<close>
+lemma vmtf_consD:
+  assumes vmtf: \<open>((ns, m, fst_As, lst_As, next_search), remove) \<in> vmtf \<A> M\<close>
+  shows \<open>((ns, m, fst_As, lst_As, next_search), remove) \<in> vmtf \<A> (L # M)\<close>
 proof -
   obtain xs' ys' where
     vmtf_ns: \<open>vmtf_ns (ys' @ xs') m ns\<close> and
     fst_As: \<open>fst_As = hd (ys' @ xs')\<close> and
     lst_As: \<open>lst_As = last (ys' @ xs')\<close> and
     next_search: \<open>next_search = option_hd xs'\<close> and
-    abs_vmtf: \<open>vmtf_\<L>\<^sub>a\<^sub>l\<^sub>l M ((set xs', set ys'), remove)\<close> and
+    abs_vmtf: \<open>vmtf_\<L>\<^sub>a\<^sub>l\<^sub>l \<A> M ((set xs', set ys'), remove)\<close> and
     notin: \<open>vmtf_ns_notin (ys' @ xs') m ns\<close> and
-    atm_A: \<open>\<forall>L\<in>atms_of \<L>\<^sub>a\<^sub>l\<^sub>l. L < length ns\<close> and
-    \<open>\<forall>L\<in>set (ys' @ xs'). L \<in> atms_of \<L>\<^sub>a\<^sub>l\<^sub>l\<close>
+    atm_A: \<open>\<forall>L\<in>atms_of (\<L>\<^sub>a\<^sub>l\<^sub>l \<A>). L < length ns\<close> and
+    \<open>\<forall>L\<in>set (ys' @ xs'). L \<in> atms_of (\<L>\<^sub>a\<^sub>l\<^sub>l \<A>)\<close>
     using vmtf unfolding vmtf_def by fast
-  moreover have \<open>vmtf_\<L>\<^sub>a\<^sub>l\<^sub>l (L # M) ((set xs', set ys'), remove)\<close>
+  moreover have \<open>vmtf_\<L>\<^sub>a\<^sub>l\<^sub>l \<A> (L # M) ((set xs', set ys'), remove)\<close>
     using abs_vmtf unfolding vmtf_\<L>\<^sub>a\<^sub>l\<^sub>l_def by auto
   ultimately have \<open>vmtf_ns (ys' @ xs') m ns \<and>
        fst_As = hd (ys' @ xs') \<and>
        lst_As = last (ys' @ xs') \<and>
        next_search = option_hd xs' \<and>
-       vmtf_\<L>\<^sub>a\<^sub>l\<^sub>l (L # M) ((set xs', set ys'), remove) \<and>
-       vmtf_ns_notin (ys' @ xs') m ns \<and> (\<forall>L\<in>atms_of \<L>\<^sub>a\<^sub>l\<^sub>l. L < length ns) \<and>
-       (\<forall>L\<in>set (ys' @ xs'). L \<in> atms_of \<L>\<^sub>a\<^sub>l\<^sub>l)\<close>
+       vmtf_\<L>\<^sub>a\<^sub>l\<^sub>l \<A> (L # M) ((set xs', set ys'), remove) \<and>
+       vmtf_ns_notin (ys' @ xs') m ns \<and> (\<forall>L\<in>atms_of (\<L>\<^sub>a\<^sub>l\<^sub>l \<A>). L < length ns) \<and>
+       (\<forall>L\<in>set (ys' @ xs'). L \<in> atms_of (\<L>\<^sub>a\<^sub>l\<^sub>l \<A>))\<close>
       by fast
   then show ?thesis
     unfolding vmtf_def by fast
@@ -1062,7 +1059,7 @@ definition (in -) vmtf_dequeue :: \<open>nat \<Rightarrow> vmtf \<Rightarrow> vm
    (ns_vmtf_dequeue L ns, m, fst_As', lst_As', next_search')))\<close>
 
 text \<open>It would be better to distinguish whether L is set in M or not.\<close>
-definition (in -) vmtf_enqueue :: \<open>(nat, nat) ann_lits \<Rightarrow> nat \<Rightarrow> vmtf_option_fst_As \<Rightarrow>  vmtf\<close> where
+definition vmtf_enqueue :: \<open>(nat, nat) ann_lits \<Rightarrow> nat \<Rightarrow> vmtf_option_fst_As \<Rightarrow>  vmtf\<close> where
 \<open>vmtf_enqueue = (\<lambda>M L (ns, m, fst_As, lst_As, next_search).
   (case fst_As of
     None \<Rightarrow> (ns[L := VMTF_Node m fst_As None], m+1, L, L,
@@ -1077,17 +1074,18 @@ definition (in -) vmtf_en_dequeue :: \<open>(nat, nat) ann_lits \<Rightarrow> na
 
 lemma abs_vmtf_ns_bump_vmtf_dequeue:
   fixes M
-  assumes vmtf:\<open>((ns, m, fst_As, lst_As, next_search), to_remove) \<in> vmtf M\<close>  and
-    L: \<open>L \<in> atms_of \<L>\<^sub>a\<^sub>l\<^sub>l\<close> and
+  assumes vmtf:\<open>((ns, m, fst_As, lst_As, next_search), to_remove) \<in> vmtf \<A> M\<close>  and
+    L: \<open>L \<in> atms_of (\<L>\<^sub>a\<^sub>l\<^sub>l \<A>)\<close> and
     dequeue: \<open>(ns', m', fst_As', lst_As', next_search') =
-       vmtf_dequeue L (ns, m, fst_As, lst_As, next_search)\<close>
+       vmtf_dequeue L (ns, m, fst_As, lst_As, next_search)\<close> and
+    \<A>\<^sub>i\<^sub>n_nempty: \<open>isasat_input_nempty \<A>\<close>
   shows \<open>\<exists>xs' ys'. vmtf_ns (ys' @ xs') m' ns' \<and> fst_As' = option_hd (ys' @ xs')
    \<and> lst_As' = option_last (ys' @ xs')
    \<and> next_search' = option_hd xs'
    \<and> next_search' = (if next_search = Some L then get_next (ns!L) else next_search)
-   \<and> vmtf_\<L>\<^sub>a\<^sub>l\<^sub>l M ((insert L (set xs'), set ys'), to_remove)
+   \<and> vmtf_\<L>\<^sub>a\<^sub>l\<^sub>l \<A> M ((insert L (set xs'), set ys'), to_remove)
    \<and> vmtf_ns_notin (ys' @ xs') m' ns' \<and>
-   L \<notin> set (ys' @ xs') \<and> (\<forall>L\<in>set (ys' @ xs'). L \<in> atms_of \<L>\<^sub>a\<^sub>l\<^sub>l)\<close>
+   L \<notin> set (ys' @ xs') \<and> (\<forall>L\<in>set (ys' @ xs'). L \<in> atms_of (\<L>\<^sub>a\<^sub>l\<^sub>l \<A>))\<close>
   unfolding vmtf_def
 proof -
   have ns': \<open>ns' = ns_vmtf_dequeue L ns\<close> and
@@ -1101,11 +1099,11 @@ proof -
     vmtf: \<open>vmtf_ns (ys @ xs) m ns\<close> and
     notin: \<open>vmtf_ns_notin (ys @ xs) m ns\<close> and
     next_search: \<open>next_search = option_hd xs\<close> and
-    abs_inv: \<open>vmtf_\<L>\<^sub>a\<^sub>l\<^sub>l M ((set xs, set ys), to_remove)\<close> and
+    abs_inv: \<open>vmtf_\<L>\<^sub>a\<^sub>l\<^sub>l \<A> M ((set xs, set ys), to_remove)\<close> and
     fst_As: \<open>fst_As = hd (ys @ xs)\<close> and
     lst_As: \<open>lst_As = last (ys @ xs)\<close> and
-    atm_A: \<open>\<forall>L\<in>atms_of \<L>\<^sub>a\<^sub>l\<^sub>l. L < length ns\<close> and
-    L_ys_xs: \<open>\<forall>L\<in>set (ys @ xs). L \<in> atms_of \<L>\<^sub>a\<^sub>l\<^sub>l\<close>
+    atm_A: \<open>\<forall>L\<in>atms_of (\<L>\<^sub>a\<^sub>l\<^sub>l \<A>). L < length ns\<close> and
+    L_ys_xs: \<open>\<forall>L\<in>set (ys @ xs). L \<in> atms_of (\<L>\<^sub>a\<^sub>l\<^sub>l \<A>)\<close>
     using vmtf unfolding vmtf_def by auto
   have [dest]: \<open>xs = [] \<Longrightarrow> ys = [] \<Longrightarrow> False\<close>
     using abs_inv \<A>\<^sub>i\<^sub>n_nempty unfolding atms_of_\<L>\<^sub>a\<^sub>l\<^sub>l_\<A>\<^sub>i\<^sub>n vmtf_\<L>\<^sub>a\<^sub>l\<^sub>l_def
@@ -1170,7 +1168,7 @@ proof -
     apply (cases \<open>ys @ xs\<close> rule: rev_cases)
     using lst_As vmtf_ns_distinct[OF vmtf] vmtf_ns_last_prev vmtf
     by (auto simp: lst_As' remove1_append simp del: distinct_append) auto
-  moreover have \<open>vmtf_\<L>\<^sub>a\<^sub>l\<^sub>l M ((insert L (set (remove1 L xs)), set (remove1 L ys)),
+  moreover have \<open>vmtf_\<L>\<^sub>a\<^sub>l\<^sub>l \<A> M ((insert L (set (remove1 L xs)), set (remove1 L ys)),
     to_remove)\<close>
     using abs_inv L dist
     unfolding vmtf_\<L>\<^sub>a\<^sub>l\<^sub>l_def by (auto dest: in_set_remove1D)
@@ -1181,11 +1179,11 @@ proof -
     subgoal using notin unfolding m'm .
     subgoal using atm_L_A .
     done
-  moreover have \<open>\<forall>L\<in>atms_of \<L>\<^sub>a\<^sub>l\<^sub>l. L < length ns'\<close>
+  moreover have \<open>\<forall>L\<in>atms_of (\<L>\<^sub>a\<^sub>l\<^sub>l \<A>). L < length ns'\<close>
     using atm_A unfolding ns' by auto
   moreover have \<open>L \<notin> set (remove1 L ys @ remove1 L xs)\<close>
     using dist by auto
-  moreover have \<open>\<forall>L\<in>set (remove1 L (ys @ xs)). L \<in> atms_of \<L>\<^sub>a\<^sub>l\<^sub>l\<close>
+  moreover have \<open>\<forall>L\<in>set (remove1 L (ys @ xs)). L \<in> atms_of (\<L>\<^sub>a\<^sub>l\<^sub>l \<A>)\<close>
     using L_ys_xs by (auto dest: in_set_remove1D)
   ultimately show ?thesis
     using next_search_L_next
@@ -1215,10 +1213,11 @@ lemma vmtf_ns_get_next_not_itself:
 lemma abs_vmtf_ns_bump_vmtf_en_dequeue:
   fixes M
   assumes
-    vmtf: \<open>((ns, m, fst_As, lst_As, next_search), to_remove) \<in> vmtf M\<close> and
-    L: \<open>L \<in> atms_of \<L>\<^sub>a\<^sub>l\<^sub>l\<close> and
-    to_remove: \<open>to_remove' \<subseteq> to_remove - {L}\<close>
-  shows \<open>(vmtf_en_dequeue M L (ns, m, fst_As, lst_As, next_search), to_remove') \<in> vmtf M\<close>
+    vmtf: \<open>((ns, m, fst_As, lst_As, next_search), to_remove) \<in> vmtf \<A> M\<close> and
+    L: \<open>L \<in> atms_of (\<L>\<^sub>a\<^sub>l\<^sub>l \<A>)\<close> and
+    to_remove: \<open>to_remove' \<subseteq> to_remove - {L}\<close> and
+    nempty: \<open>isasat_input_nempty \<A>\<close>
+  shows \<open>(vmtf_en_dequeue M L (ns, m, fst_As, lst_As, next_search), to_remove') \<in> vmtf \<A> M\<close>
   unfolding vmtf_def
 proof clarify
   fix xxs yys zzs ns' m' fst_As' lst_As' next_search'
@@ -1228,11 +1227,11 @@ proof clarify
     vmtf_ns: \<open>vmtf_ns (ys @ xs) m ns\<close> and
     notin: \<open>vmtf_ns_notin (ys @ xs) m ns\<close> and
     next_search: \<open>next_search = option_hd xs\<close> and
-    abs_inv: \<open>vmtf_\<L>\<^sub>a\<^sub>l\<^sub>l M ((set xs, set ys), to_remove)\<close> and
+    abs_inv: \<open>vmtf_\<L>\<^sub>a\<^sub>l\<^sub>l \<A> M ((set xs, set ys), to_remove)\<close> and
     fst_As: \<open>fst_As = hd (ys @ xs)\<close> and
     lst_As: \<open>lst_As = last (ys @ xs)\<close> and
-    atm_A: \<open>\<forall>L\<in>atms_of \<L>\<^sub>a\<^sub>l\<^sub>l. L < length ns\<close> and
-    ys_xs_\<L>\<^sub>a\<^sub>l\<^sub>l: \<open>\<forall>L\<in>set (ys @ xs). L \<in> atms_of \<L>\<^sub>a\<^sub>l\<^sub>l\<close>
+    atm_A: \<open>\<forall>L\<in>atms_of (\<L>\<^sub>a\<^sub>l\<^sub>l \<A>). L < length ns\<close> and
+    ys_xs_\<L>\<^sub>a\<^sub>l\<^sub>l: \<open>\<forall>L\<in>set (ys @ xs). L \<in> atms_of (\<L>\<^sub>a\<^sub>l\<^sub>l \<A>)\<close>
     using assms unfolding vmtf_def by auto
   have atm_L_A: \<open>L < length ns\<close>
     using atm_A L by blast
@@ -1247,11 +1246,11 @@ proof clarify
     next_searchd_hd: \<open>next_searchd = option_hd xs'\<close> and
     next_searchd_L_next:
       \<open>next_searchd = (if next_search = Some L then get_next (ns!L) else next_search)\<close> and
-    abs_l: \<open>vmtf_\<L>\<^sub>a\<^sub>l\<^sub>l M ((insert L (set xs'), set ys'), to_remove)\<close>  and
+    abs_l: \<open>vmtf_\<L>\<^sub>a\<^sub>l\<^sub>l \<A> M ((insert L (set xs'), set ys'), to_remove)\<close>  and
     not_in: \<open>vmtf_ns_notin (ys' @ xs') md nsd\<close> and
     L_xs'_ys': \<open>L \<notin> set (ys' @ xs')\<close> and
-    L_xs'_ys'_\<L>\<^sub>a\<^sub>l\<^sub>l: \<open>\<forall>L\<in>set (ys' @ xs'). L \<in> atms_of \<L>\<^sub>a\<^sub>l\<^sub>l\<close>
-    using abs_vmtf_ns_bump_vmtf_dequeue[OF vmtf L de[symmetric]] by blast
+    L_xs'_ys'_\<L>\<^sub>a\<^sub>l\<^sub>l: \<open>\<forall>L\<in>set (ys' @ xs'). L \<in> atms_of (\<L>\<^sub>a\<^sub>l\<^sub>l \<A>)\<close>
+    using abs_vmtf_ns_bump_vmtf_dequeue[OF vmtf L de[symmetric] nempty] by blast
 
   have [simp]: \<open>length ns' = length ns\<close>  \<open>length nsd = length ns\<close>
     using dequeue de unfolding vmtf_en_dequeue_def comp_def vmtf_dequeue_def
@@ -1260,11 +1259,11 @@ proof clarify
     using de unfolding vmtf_dequeue_def by auto
   have [simp]: \<open>fst_As = L\<close> if \<open>ys' = []\<close> and \<open>xs' = []\<close>
     proof -
-      have 1: \<open>set_mset \<A>\<^sub>i\<^sub>n = {L}\<close>
+      have 1: \<open>set_mset \<A> = {L}\<close>
         using abs_l unfolding that vmtf_\<L>\<^sub>a\<^sub>l\<^sub>l_def by (auto simp: atms_of_\<L>\<^sub>a\<^sub>l\<^sub>l_\<A>\<^sub>i\<^sub>n)
       show ?thesis
-        using vmtf_ns_distinct[OF vmtf_ns] ys_xs_\<L>\<^sub>a\<^sub>l\<^sub>l abs_inv vmtf_\<L>\<^sub>a\<^sub>l\<^sub>l_def
-        unfolding atms_of_\<L>\<^sub>a\<^sub>l\<^sub>l_\<A>\<^sub>i\<^sub>n 1 fst_As
+        using vmtf_ns_distinct[OF vmtf_ns] ys_xs_\<L>\<^sub>a\<^sub>l\<^sub>l abs_inv 
+        unfolding atms_of_\<L>\<^sub>a\<^sub>l\<^sub>l_\<A>\<^sub>i\<^sub>n 1 fst_As vmtf_\<L>\<^sub>a\<^sub>l\<^sub>l_def
         by (cases \<open>ys @ xs\<close>)  auto
     qed
     have fst_As': \<open>fst_As' = L\<close> and m': \<open>m' = md + 1\<close> and
@@ -1274,11 +1273,11 @@ proof clarify
       by (auto simp add: vmtf_enqueue_def split: option.splits)
     have \<open>lst_As = L\<close> if \<open>ys' = []\<close> and \<open>xs' = []\<close>
     proof -
-      have 1: \<open>set_mset \<A>\<^sub>i\<^sub>n = {L}\<close>
+      have 1: \<open>set_mset \<A> = {L}\<close>
         using abs_l unfolding that vmtf_\<L>\<^sub>a\<^sub>l\<^sub>l_def by (auto simp: atms_of_\<L>\<^sub>a\<^sub>l\<^sub>l_\<A>\<^sub>i\<^sub>n)
       then have \<open>set (ys @ xs) = {L} \<close>
-        using vmtf_ns_distinct[OF vmtf_ns] ys_xs_\<L>\<^sub>a\<^sub>l\<^sub>l abs_inv vmtf_\<L>\<^sub>a\<^sub>l\<^sub>l_def
-        unfolding atms_of_\<L>\<^sub>a\<^sub>l\<^sub>l_\<A>\<^sub>i\<^sub>n 1 fst_As
+        using vmtf_ns_distinct[OF vmtf_ns] ys_xs_\<L>\<^sub>a\<^sub>l\<^sub>l abs_inv
+        unfolding atms_of_\<L>\<^sub>a\<^sub>l\<^sub>l_\<A>\<^sub>i\<^sub>n 1 fst_As vmtf_\<L>\<^sub>a\<^sub>l\<^sub>l_def
         by auto
       then have \<open>ys @ xs = [L]\<close>
         using vmtf_ns_distinct[OF vmtf_ns] ys_xs_\<L>\<^sub>a\<^sub>l\<^sub>l abs_inv vmtf_\<L>\<^sub>a\<^sub>l\<^sub>l_def
@@ -1334,10 +1333,10 @@ proof clarify
        fst_As' = hd (ys' @ xs') \<and>
        lst_As' = last (ys' @ xs') \<and>
        next_search' = option_hd xs' \<and>
-       vmtf_\<L>\<^sub>a\<^sub>l\<^sub>l M ((set xs', set ys'), to_remove') \<and>
+       vmtf_\<L>\<^sub>a\<^sub>l\<^sub>l \<A> M ((set xs', set ys'), to_remove') \<and>
        vmtf_ns_notin (ys' @ xs') m' ns' \<and>
-       (\<forall>L\<in>atms_of \<L>\<^sub>a\<^sub>l\<^sub>l. L < length ns') \<and>
-       (\<forall>L\<in>set (ys' @ xs'). L \<in> atms_of \<L>\<^sub>a\<^sub>l\<^sub>l)\<close>
+       (\<forall>L\<in>atms_of (\<L>\<^sub>a\<^sub>l\<^sub>l \<A>). L < length ns') \<and>
+       (\<forall>L\<in>set (ys' @ xs'). L \<in> atms_of (\<L>\<^sub>a\<^sub>l\<^sub>l \<A>))\<close>
   proof cases
     case defined
     have L_in_M: \<open>L \<in> atm_of ` lits_of_l M\<close>
@@ -1349,7 +1348,7 @@ proof clarify
     have next_searchd:
       \<open>next_searchd = (if next_search = Some L then get_next (ns ! L) else next_search)\<close>
       using de by (auto simp: vmtf_dequeue_def)
-    have abs': \<open>vmtf_\<L>\<^sub>a\<^sub>l\<^sub>l M  ((set xs', insert L (set ys')), to_remove')\<close>
+    have abs': \<open>vmtf_\<L>\<^sub>a\<^sub>l\<^sub>l \<A> M  ((set xs', insert L (set ys')), to_remove')\<close>
       using abs_l to_remove L_in_M L_xs'_ys' unfolding vmtf_\<L>\<^sub>a\<^sub>l\<^sub>l_def
       by (auto 5 5 dest: in_diffD)
 
@@ -1395,7 +1394,7 @@ proof clarify
         subgoal by linarith
         done
     qed
-    have L_xs'_ys'_\<L>\<^sub>a\<^sub>l\<^sub>l': \<open>\<forall>L'\<in>set ((L # ys') @ xs'). L' \<in> atms_of \<L>\<^sub>a\<^sub>l\<^sub>l\<close>
+    have L_xs'_ys'_\<L>\<^sub>a\<^sub>l\<^sub>l': \<open>\<forall>L'\<in>set ((L # ys') @ xs'). L' \<in> atms_of (\<L>\<^sub>a\<^sub>l\<^sub>l \<A>)\<close>
       using L L_xs'_ys'_\<L>\<^sub>a\<^sub>l\<^sub>l by auto
     have next_search'_xs': \<open>next_search' = option_hd xs'\<close>
       using next_searchd_L_next next_search' next_searchd_hd lst_As' fst_Asd
@@ -1414,7 +1413,7 @@ proof clarify
     have next_searchd:
       \<open>next_searchd = (if next_search = Some L then get_next (ns ! L) else next_search)\<close>
       using de by (auto simp: vmtf_dequeue_def)
-    have abs': \<open>vmtf_\<L>\<^sub>a\<^sub>l\<^sub>l M  ((insert L (set (ys' @ xs')), set []), to_remove')\<close>
+    have abs': \<open>vmtf_\<L>\<^sub>a\<^sub>l\<^sub>l \<A> M  ((insert L (set (ys' @ xs')), set []), to_remove')\<close>
       using abs_l to_remove L_xs'_ys' unfolding vmtf_\<L>\<^sub>a\<^sub>l\<^sub>l_def
       by (auto 5 5 dest: in_diffD)
 
@@ -1460,7 +1459,7 @@ proof clarify
         subgoal by linarith
         done
     qed
-    have L_xs'_ys'_\<L>\<^sub>a\<^sub>l\<^sub>l': \<open>\<forall>L'\<in>set ((L # ys') @ xs'). L' \<in> atms_of \<L>\<^sub>a\<^sub>l\<^sub>l\<close>
+    have L_xs'_ys'_\<L>\<^sub>a\<^sub>l\<^sub>l': \<open>\<forall>L'\<in>set ((L # ys') @ xs'). L' \<in> atms_of (\<L>\<^sub>a\<^sub>l\<^sub>l \<A>)\<close>
       using L L_xs'_ys'_\<L>\<^sub>a\<^sub>l\<^sub>l by auto
     show ?thesis
       apply (rule exI[of _ \<open>(L # ys') @ xs'\<close>])
@@ -1475,10 +1474,11 @@ qed
 lemma abs_vmtf_ns_bump_vmtf_en_dequeue':
   fixes M
   assumes
-    vmtf: \<open>(vm, to_remove) \<in> vmtf M\<close> and
-    L: \<open>L \<in> atms_of \<L>\<^sub>a\<^sub>l\<^sub>l\<close> and
-    to_remove: \<open>to_remove' \<subseteq> to_remove - {L}\<close>
-  shows \<open>(vmtf_en_dequeue M L vm, to_remove') \<in> vmtf M\<close>
+    vmtf: \<open>(vm, to_remove) \<in> vmtf \<A> M\<close> and
+    L: \<open>L \<in> atms_of (\<L>\<^sub>a\<^sub>l\<^sub>l \<A>)\<close> and
+    to_remove: \<open>to_remove' \<subseteq> to_remove - {L}\<close> and
+    nempty: \<open>isasat_input_nempty \<A>\<close>
+  shows \<open>(vmtf_en_dequeue M L vm, to_remove') \<in> vmtf \<A> M\<close>
   using abs_vmtf_ns_bump_vmtf_en_dequeue assms by (cases vm) blast
 
 definition (in -) vmtf_unset :: \<open>nat \<Rightarrow> vmtf_remove_int \<Rightarrow> vmtf_remove_int\<close> where
@@ -1491,9 +1491,9 @@ lemma vmtf_atm_of_ys_iff:
   assumes
     vmtf_ns: \<open>vmtf_ns (ys' @ xs') m ns\<close> and
     next_search: \<open>next_search = option_hd xs'\<close> and
-    abs_vmtf: \<open>vmtf_\<L>\<^sub>a\<^sub>l\<^sub>l M ((set xs', set ys'), to_remove)\<close> and
-    L: \<open>L \<in> atms_of \<L>\<^sub>a\<^sub>l\<^sub>l\<close>
-  shows \<open>L \<in> set ys' \<longleftrightarrow> next_search = None \<or> stamp (ns ! (the next_search)) < stamp (ns ! L)\<close>
+    abs_vmtf: \<open>vmtf_\<L>\<^sub>a\<^sub>l\<^sub>l \<A> M ((set xs', set ys'), to_remove)\<close> and
+    L: \<open>L \<in> atms_of (\<L>\<^sub>a\<^sub>l\<^sub>l \<A>)\<close>
+    shows \<open>L \<in> set ys' \<longleftrightarrow> next_search = None \<or> stamp (ns ! (the next_search)) < stamp (ns ! L)\<close>
 proof -
   let ?xs' = \<open>set xs'\<close>
   let ?ys' = \<open>set ys'\<close>
@@ -1533,25 +1533,26 @@ qed
 
 lemma vmtf_\<L>\<^sub>a\<^sub>l\<^sub>l_to_remove_mono:
   assumes
-    \<open>vmtf_\<L>\<^sub>a\<^sub>l\<^sub>l M ((a, b), to_remove)\<close> and
+    \<open>vmtf_\<L>\<^sub>a\<^sub>l\<^sub>l \<A> M ((a, b), to_remove)\<close> and
     \<open>to_remove' \<subseteq> to_remove\<close>
-  shows \<open>vmtf_\<L>\<^sub>a\<^sub>l\<^sub>l M ((a, b), to_remove')\<close>
+  shows \<open>vmtf_\<L>\<^sub>a\<^sub>l\<^sub>l \<A> M ((a, b), to_remove')\<close>
   using assms unfolding vmtf_\<L>\<^sub>a\<^sub>l\<^sub>l_def by (auto simp: mset_subset_eqD)
 
 lemma abs_vmtf_ns_unset_vmtf_unset:
-  assumes vmtf:\<open>((ns, m, fst_As, lst_As, next_search), to_remove) \<in> vmtf M\<close> and L_N: \<open>L \<in> atms_of \<L>\<^sub>a\<^sub>l\<^sub>l\<close> and
+  assumes vmtf:\<open>((ns, m, fst_As, lst_As, next_search), to_remove) \<in> vmtf \<A> M\<close> and
+  L_N: \<open>L \<in> atms_of (\<L>\<^sub>a\<^sub>l\<^sub>l \<A>)\<close> and
     to_remove: \<open>to_remove' \<subseteq> to_remove\<close>
-  shows \<open>(vmtf_unset L ((ns, m, fst_As, lst_As, next_search), to_remove')) \<in> vmtf M\<close> (is \<open>?S \<in> _\<close>)
+  shows \<open>(vmtf_unset L ((ns, m, fst_As, lst_As, next_search), to_remove')) \<in> vmtf \<A> M\<close> (is \<open>?S \<in> _\<close>)
 proof -
   obtain xs' ys' where
     vmtf_ns: \<open>vmtf_ns (ys' @ xs') m ns\<close> and
     fst_As: \<open>fst_As = hd (ys' @ xs')\<close> and
     lst_As: \<open>lst_As = last (ys' @ xs')\<close> and
     next_search: \<open>next_search = option_hd xs'\<close> and
-    abs_vmtf: \<open>vmtf_\<L>\<^sub>a\<^sub>l\<^sub>l M ((set xs', set ys'), to_remove)\<close> and
+    abs_vmtf: \<open>vmtf_\<L>\<^sub>a\<^sub>l\<^sub>l \<A> M ((set xs', set ys'), to_remove)\<close> and
     notin: \<open>vmtf_ns_notin (ys' @ xs') m ns\<close> and
-    atm_A: \<open>\<forall>L\<in>atms_of \<L>\<^sub>a\<^sub>l\<^sub>l. L < length ns\<close> and
-    L_ys'_xs'_\<L>\<^sub>a\<^sub>l\<^sub>l: \<open>\<forall>L\<in>set (ys' @ xs'). L \<in> atms_of \<L>\<^sub>a\<^sub>l\<^sub>l\<close>
+    atm_A: \<open>\<forall>L\<in>atms_of (\<L>\<^sub>a\<^sub>l\<^sub>l \<A>). L < length ns\<close> and
+    L_ys'_xs'_\<L>\<^sub>a\<^sub>l\<^sub>l: \<open>\<forall>L\<in>set (ys' @ xs'). L \<in> atms_of (\<L>\<^sub>a\<^sub>l\<^sub>l \<A>)\<close>
     using vmtf unfolding vmtf_def by fast
   obtain ns' m' fst_As' next_search' to_remove'' lst_As' where
     S: \<open>?S = ((ns', m', fst_As', lst_As', next_search'), to_remove'')\<close>
@@ -1567,14 +1568,14 @@ proof -
        fst_As' = hd (ys' @ xs') \<and>
        lst_As' = last (ys' @ xs') \<and>
        next_search' = option_hd xs' \<and>
-       vmtf_\<L>\<^sub>a\<^sub>l\<^sub>l M ((set xs', set ys'), to_remove'') \<and>
-       vmtf_ns_notin (ys' @ xs') m' ns' \<and> (\<forall>L\<in>atms_of \<L>\<^sub>a\<^sub>l\<^sub>l. L < length ns') \<and>
-       (\<forall>L\<in>set (ys' @ xs'). L \<in> atms_of \<L>\<^sub>a\<^sub>l\<^sub>l)\<close>
+       vmtf_\<L>\<^sub>a\<^sub>l\<^sub>l \<A> M ((set xs', set ys'), to_remove'') \<and>
+       vmtf_ns_notin (ys' @ xs') m' ns' \<and> (\<forall>L\<in>atms_of (\<L>\<^sub>a\<^sub>l\<^sub>l \<A>). L < length ns') \<and>
+       (\<forall>L\<in>set (ys' @ xs'). L \<in> atms_of (\<L>\<^sub>a\<^sub>l\<^sub>l \<A>))\<close>
   proof (cases \<open>L \<in> set xs'\<close>)
     case True
     then have C: \<open>\<not>(next_search = None \<or> stamp (ns ! the next_search) < stamp (ns ! L))\<close>
       by (subst L_ys'_iff[symmetric]) (use L_ys'_xs' in auto)
-    have abs_vmtf: \<open>vmtf_\<L>\<^sub>a\<^sub>l\<^sub>l M ((set xs', set ys'), to_remove'')\<close>
+    have abs_vmtf: \<open>vmtf_\<L>\<^sub>a\<^sub>l\<^sub>l \<A> M ((set xs', set ys'), to_remove'')\<close>
     apply (rule vmtf_\<L>\<^sub>a\<^sub>l\<^sub>l_to_remove_mono)
     apply (rule abs_vmtf)
     using to_remove S unfolding vmtf_unset_def by (auto simp: C)
@@ -1618,15 +1619,15 @@ proof -
     moreover have \<open>next_search' = option_hd ?xs'\<close>
       by auto
     moreover {
-      have \<open>vmtf_\<L>\<^sub>a\<^sub>l\<^sub>l M ((set ?xs', set ?ys'), to_remove)\<close>
+      have \<open>vmtf_\<L>\<^sub>a\<^sub>l\<^sub>l \<A> M ((set ?xs', set ?ys'), to_remove)\<close>
         using abs_vmtf vmtf_ns_distinct[OF vmtf_ns] unfolding vmtf_\<L>\<^sub>a\<^sub>l\<^sub>l_def ys'_y_x
         by auto
-      then have \<open>vmtf_\<L>\<^sub>a\<^sub>l\<^sub>l M ((set ?xs', set ?ys'), to_remove')\<close>
+      then have \<open>vmtf_\<L>\<^sub>a\<^sub>l\<^sub>l \<A> M ((set ?xs', set ?ys'), to_remove')\<close>
         by (rule vmtf_\<L>\<^sub>a\<^sub>l\<^sub>l_to_remove_mono) (use to_remove in auto)
       }
     moreover have \<open>vmtf_ns_notin (?ys' @ ?xs') m ns\<close>
       using notin unfolding ys'_y_x by simp
-    moreover have \<open>\<forall>L\<in>set (?ys' @ ?xs'). L \<in> atms_of \<L>\<^sub>a\<^sub>l\<^sub>l\<close>
+    moreover have \<open>\<forall>L\<in>set (?ys' @ ?xs'). L \<in> atms_of (\<L>\<^sub>a\<^sub>l\<^sub>l \<A>)\<close>
       using L_ys'_xs'_\<L>\<^sub>a\<^sub>l\<^sub>l unfolding ys'_y_x by auto
     ultimately show ?thesis
       using S False atm_A unfolding vmtf_unset_def L_ys'_xs'[symmetric]
@@ -1653,26 +1654,26 @@ lemma (in -) vmtf_dequeue_pre_alt_def:
       (auto simp: vmtf_dequeue_pre_def intro!: ext)
   done
 
-definition (in isasat_input_ops) vmtf_en_dequeue_pre :: \<open>((nat, nat) ann_lits \<times> nat) \<times> vmtf \<Rightarrow> bool\<close> where
-  \<open>vmtf_en_dequeue_pre = (\<lambda>((M, L),(ns,m,fst_As, lst_As, next_search)). L < length ns \<and> vmtf_dequeue_pre (L, ns) \<and>
+definition vmtf_en_dequeue_pre :: \<open>nat multiset \<Rightarrow> ((nat, nat) ann_lits \<times> nat) \<times> vmtf \<Rightarrow> bool\<close> where
+  \<open>vmtf_en_dequeue_pre \<A> = (\<lambda>((M, L),(ns,m,fst_As, lst_As, next_search)).
+       L < length ns \<and> vmtf_dequeue_pre (L, ns) \<and>
        fst_As < length ns \<and> (get_next (ns ! fst_As) \<noteq> None \<longrightarrow> get_prev (ns ! lst_As) \<noteq> None) \<and>
        (get_next (ns ! fst_As) = None \<longrightarrow> fst_As = lst_As) \<and>
        m+1 \<le> uint64_max \<and>
-       Pos L \<in># \<L>\<^sub>a\<^sub>l\<^sub>l)\<close>
+       Pos L \<in># \<L>\<^sub>a\<^sub>l\<^sub>l \<A>)\<close>
 
 definition (in -) distinct_atoms_rel
   :: \<open>(('v list \<times> 'v set) \<times> 'v set) set\<close>
 where
   \<open>distinct_atoms_rel = {((C, h), D). set C = D \<and> h = D \<and> distinct C}\<close>
 
-definition (in isasat_input_ops) atoms_hash_rel :: \<open>(bool list \<times> nat set) set\<close> where
-  \<open>atoms_hash_rel = {(C, D). (\<forall>L \<in> D. L < length C) \<and> (\<forall>L < length C. C ! L \<longleftrightarrow> L \<in> D) \<and>
-     (\<forall>L \<in># \<A>\<^sub>i\<^sub>n. L < length C)}\<close>
+definition atoms_hash_rel :: \<open>(bool list \<times> nat set) set\<close> where
+  \<open>atoms_hash_rel = {(C, D). (\<forall>L \<in> D. L < length C) \<and> (\<forall>L < length C. C ! L \<longleftrightarrow> L \<in> D)}\<close>
 
-definition (in isasat_input_ops) atoms_hash_assn :: \<open>nat set \<Rightarrow> bool array \<Rightarrow> assn\<close> where
+definition atoms_hash_assn :: \<open>nat set \<Rightarrow> bool array \<Rightarrow> assn\<close> where
   \<open>atoms_hash_assn = hr_comp (array_assn bool_assn) atoms_hash_rel\<close>
 
-definition (in isasat_input_ops) distinct_atoms_assn where
+definition distinct_atoms_assn where
   \<open>distinct_atoms_assn = hr_comp (arl_assn uint32_nat_assn *a atoms_hash_assn) distinct_atoms_rel\<close>
 
 
@@ -1681,33 +1682,34 @@ lemma (in -) id_reorder_remove:
   unfolding reorder_remove_def by (intro frefI nres_relI) auto
 
 lemma vmtf_vmtf_en_dequeue_pre_to_remove:
-  assumes vmtf: \<open>((ns, m, fst_As, lst_As, next_search), to_remove) \<in> vmtf M\<close> and
+  assumes vmtf: \<open>((ns, m, fst_As, lst_As, next_search), to_remove) \<in> vmtf \<A> M\<close> and
     i: \<open>A \<in> to_remove\<close> and
-    m_le:  \<open>m + 1 \<le> uint64_max\<close>
-  shows \<open>vmtf_en_dequeue_pre ((M, A), (ns, m, fst_As, lst_As, next_search))\<close>
+    m_le:  \<open>m + 1 \<le> uint64_max\<close> and
+    nempty: \<open>isasat_input_nempty \<A>\<close>
+  shows \<open>vmtf_en_dequeue_pre \<A> ((M, A), (ns, m, fst_As, lst_As, next_search))\<close>
 proof -
   obtain xs' ys' where
     vmtf_ns: \<open>vmtf_ns (ys' @ xs') m ns\<close> and
     fst_As: \<open>fst_As = hd (ys' @ xs')\<close> and
     lst_As: \<open>lst_As = last (ys' @ xs')\<close> and
     next_search: \<open>next_search = option_hd xs'\<close> and
-    abs_vmtf: \<open>vmtf_\<L>\<^sub>a\<^sub>l\<^sub>l M ((set xs', set ys'), to_remove)\<close> and
+    abs_vmtf: \<open>vmtf_\<L>\<^sub>a\<^sub>l\<^sub>l \<A> M ((set xs', set ys'), to_remove)\<close> and
     notin: \<open>vmtf_ns_notin (ys' @ xs') m ns\<close> and
-    atm_A: \<open>\<forall>L\<in>atms_of \<L>\<^sub>a\<^sub>l\<^sub>l. L < length ns\<close> and
-    L_ys'_xs'_\<L>\<^sub>a\<^sub>l\<^sub>l: \<open>\<forall>L\<in>set (ys' @ xs'). L \<in> atms_of \<L>\<^sub>a\<^sub>l\<^sub>l\<close>
+    atm_A: \<open>\<forall>L\<in>atms_of (\<L>\<^sub>a\<^sub>l\<^sub>l \<A>). L < length ns\<close> and
+    L_ys'_xs'_\<L>\<^sub>a\<^sub>l\<^sub>l: \<open>\<forall>L\<in>set (ys' @ xs'). L \<in> atms_of (\<L>\<^sub>a\<^sub>l\<^sub>l \<A>)\<close>
     using vmtf unfolding vmtf_def by fast
   have [dest]: False if \<open>ys' = []\<close> and \<open>xs' = []\<close>
   proof -
-    have 1: \<open>set_mset \<A>\<^sub>i\<^sub>n = {}\<close>
+    have 1: \<open>set_mset \<A> = {}\<close>
       using abs_vmtf unfolding that vmtf_\<L>\<^sub>a\<^sub>l\<^sub>l_def by (auto simp: atms_of_\<L>\<^sub>a\<^sub>l\<^sub>l_\<A>\<^sub>i\<^sub>n)
     then show ?thesis
-      using \<A>\<^sub>i\<^sub>n_nempty by auto
+      using nempty by auto
   qed
 
-  have \<open>A \<in> atms_of \<L>\<^sub>a\<^sub>l\<^sub>l\<close>
+  have \<open>A \<in> atms_of (\<L>\<^sub>a\<^sub>l\<^sub>l \<A>)\<close>
     using abs_vmtf i unfolding vmtf_\<L>\<^sub>a\<^sub>l\<^sub>l_def by auto
   then have remove_i_le_A: \<open>A < length ns\<close> and
-    i_L: \<open>Pos A \<in># \<L>\<^sub>a\<^sub>l\<^sub>l\<close>
+    i_L: \<open>Pos A \<in># \<L>\<^sub>a\<^sub>l\<^sub>l \<A>\<close>
     using atm_A by (auto simp: in_\<L>\<^sub>a\<^sub>l\<^sub>l_atm_of_\<A>\<^sub>i\<^sub>n atms_of_def)
   moreover have \<open>fst_As < length ns\<close>
     using fst_As atm_A L_ys'_xs'_\<L>\<^sub>a\<^sub>l\<^sub>l by (cases ys'; cases xs') auto
@@ -1730,7 +1732,7 @@ proof -
       case True
       then obtain zs zs' where zs: \<open>ys' @ xs' = zs' @ [A] @ zs\<close>
         using split_list by fastforce
-      moreover have \<open>set (ys' @ xs') = atms_of \<L>\<^sub>a\<^sub>l\<^sub>l\<close>
+      moreover have \<open>set (ys' @ xs') = atms_of (\<L>\<^sub>a\<^sub>l\<^sub>l \<A>)\<close>
         using abs_vmtf unfolding vmtf_\<L>\<^sub>a\<^sub>l\<^sub>l_def by auto
       ultimately show ?thesis
         using vmtf_ns_last_mid_get_next_option_hd[of zs' A zs m ns] vmtf_ns atm_A get_next
@@ -1745,7 +1747,7 @@ proof -
       case True
       then obtain zs zs' where zs: \<open>ys' @ xs' = zs' @ [A] @ zs\<close>
         using split_list by fastforce
-      moreover have \<open>set (ys' @ xs') = atms_of \<L>\<^sub>a\<^sub>l\<^sub>l\<close>
+      moreover have \<open>set (ys' @ xs') = atms_of (\<L>\<^sub>a\<^sub>l\<^sub>l \<A>)\<close>
         using abs_vmtf unfolding vmtf_\<L>\<^sub>a\<^sub>l\<^sub>l_def by auto
       ultimately show ?thesis
         using vmtf_ns_last_mid_get_prev_option_last[of zs' A zs m ns] vmtf_ns atm_A get_prev
@@ -1765,15 +1767,16 @@ proof -
 qed
 
 lemma vmtf_vmtf_en_dequeue_pre_to_remove':
-  assumes vmtf: \<open>(vm, to_remove) \<in> vmtf M\<close> and
-    i: \<open>A \<in> to_remove\<close> and \<open>fst (snd vm) + 1 \<le> uint64_max\<close>
-  shows \<open>vmtf_en_dequeue_pre ((M, A), vm)\<close>
+  assumes vmtf: \<open>(vm, to_remove) \<in> vmtf \<A> M\<close> and
+    i: \<open>A \<in> to_remove\<close> and \<open>fst (snd vm) + 1 \<le> uint64_max\<close> and
+    A: \<open>isasat_input_nempty \<A>\<close>
+  shows \<open>vmtf_en_dequeue_pre \<A> ((M, A), vm)\<close>
   using vmtf_vmtf_en_dequeue_pre_to_remove assms
   by (cases vm) auto
 
 lemma wf_vmtf_get_next:
-  assumes vmtf: \<open>((ns, m, fst_As, lst_As, next_search), to_remove) \<in> vmtf M\<close>
-  shows \<open>wf {(get_next (ns ! the a), a) |a. a \<noteq> None \<and> the a \<in> atms_of \<L>\<^sub>a\<^sub>l\<^sub>l}\<close> (is \<open>wf ?R\<close>)
+  assumes vmtf: \<open>((ns, m, fst_As, lst_As, next_search), to_remove) \<in> vmtf \<A> M\<close>
+  shows \<open>wf {(get_next (ns ! the a), a) |a. a \<noteq> None \<and> the a \<in> atms_of (\<L>\<^sub>a\<^sub>l\<^sub>l \<A>)}\<close> (is \<open>wf ?R\<close>)
 proof (rule ccontr)
   assume \<open>\<not> ?thesis\<close>
   then obtain f where
@@ -1785,9 +1788,9 @@ proof (rule ccontr)
     fst_As: \<open>fst_As = hd (ys' @ xs')\<close> and
     lst_As: \<open>lst_As = last (ys' @ xs')\<close> and
     next_search: \<open>next_search = option_hd xs'\<close> and
-    abs_vmtf: \<open>vmtf_\<L>\<^sub>a\<^sub>l\<^sub>l M ((set xs', set ys'), to_remove)\<close> and
+    abs_vmtf: \<open>vmtf_\<L>\<^sub>a\<^sub>l\<^sub>l \<A> M ((set xs', set ys'), to_remove)\<close> and
     notin: \<open>vmtf_ns_notin (ys' @ xs') m ns\<close> and
-    atm_A: \<open>\<forall>L\<in>atms_of \<L>\<^sub>a\<^sub>l\<^sub>l. L < length ns\<close>
+    atm_A: \<open>\<forall>L\<in>atms_of (\<L>\<^sub>a\<^sub>l\<^sub>l \<A>). L < length ns\<close>
     using vmtf unfolding vmtf_def by fast
   let ?f0 = \<open>the (f 0)\<close>
   have f_None: \<open>f i \<noteq> None\<close> for i
@@ -1852,10 +1855,10 @@ qed
 
 lemma vmtf_next_search_take_next:
   assumes
-    vmtf: \<open>((ns, m, fst_As, lst_As, next_search), to_remove) \<in> vmtf M\<close> and
+    vmtf: \<open>((ns, m, fst_As, lst_As, next_search), to_remove) \<in> vmtf \<A> M\<close> and
     n: \<open>next_search \<noteq> None\<close> and
     def_n: \<open>defined_lit M (Pos (the next_search))\<close>
-  shows \<open>((ns, m, fst_As, lst_As, get_next (ns!the next_search)), to_remove) \<in> vmtf M\<close>
+  shows \<open>((ns, m, fst_As, lst_As, get_next (ns!the next_search)), to_remove) \<in> vmtf \<A> M\<close>
   unfolding vmtf_def
 proof clarify
   obtain xs' ys' where
@@ -1863,10 +1866,10 @@ proof clarify
     fst_As: \<open>fst_As = hd (ys' @ xs')\<close> and
     lst_As: \<open>lst_As = last (ys' @ xs')\<close> and
     next_search: \<open>next_search = option_hd xs'\<close> and
-    abs_vmtf: \<open>vmtf_\<L>\<^sub>a\<^sub>l\<^sub>l M ((set xs', set ys'), to_remove)\<close> and
+    abs_vmtf: \<open>vmtf_\<L>\<^sub>a\<^sub>l\<^sub>l \<A> M ((set xs', set ys'), to_remove)\<close> and
     notin: \<open>vmtf_ns_notin (ys' @ xs') m ns\<close> and
-    atm_A: \<open>\<forall>L\<in>atms_of \<L>\<^sub>a\<^sub>l\<^sub>l. L < length ns\<close> and
-    ys'_xs'_\<L>\<^sub>a\<^sub>l\<^sub>l: \<open>\<forall>L\<in>set (ys' @ xs'). L \<in> atms_of \<L>\<^sub>a\<^sub>l\<^sub>l\<close>
+    atm_A: \<open>\<forall>L\<in>atms_of (\<L>\<^sub>a\<^sub>l\<^sub>l \<A>). L < length ns\<close> and
+    ys'_xs'_\<L>\<^sub>a\<^sub>l\<^sub>l: \<open>\<forall>L\<in>set (ys' @ xs'). L \<in> atms_of (\<L>\<^sub>a\<^sub>l\<^sub>l \<A>)\<close>
     using vmtf unfolding vmtf_def by fast
   let ?xs' = \<open>tl xs'\<close>
   let ?ys' = \<open>ys' @ [hd xs']\<close>
@@ -1884,35 +1887,35 @@ proof clarify
   moreover {
     have [dest]: \<open>defined_lit M (Pos a) \<Longrightarrow> a \<in> atm_of ` lits_of_l M\<close> for a
       by (auto simp: defined_lit_map lits_of_def)
-    have \<open>vmtf_\<L>\<^sub>a\<^sub>l\<^sub>l M ((set ?xs', set ?ys'), to_remove)\<close>
+    have \<open>vmtf_\<L>\<^sub>a\<^sub>l\<^sub>l \<A> M ((set ?xs', set ?ys'), to_remove)\<close>
       using abs_vmtf def_n next_search n vmtf_ns_distinct[OF vmtf_ns]
       unfolding vmtf_\<L>\<^sub>a\<^sub>l\<^sub>l_def
       by (cases xs') auto }
   moreover have \<open>vmtf_ns_notin (?ys' @ ?xs') m ns\<close>
     using notin by auto
-  moreover have \<open>\<forall>L\<in>set (?ys' @ ?xs'). L \<in> atms_of \<L>\<^sub>a\<^sub>l\<^sub>l\<close>
+  moreover have \<open>\<forall>L\<in>set (?ys' @ ?xs'). L \<in> atms_of (\<L>\<^sub>a\<^sub>l\<^sub>l \<A>)\<close>
     using ys'_xs'_\<L>\<^sub>a\<^sub>l\<^sub>l by auto
   ultimately show \<open>\<exists>xs' ys'. vmtf_ns (ys' @ xs') m ns \<and>
           fst_As = hd (ys' @ xs') \<and>
           lst_As = last (ys' @ xs') \<and>
           get_next (ns ! the next_search) = option_hd xs' \<and>
-          vmtf_\<L>\<^sub>a\<^sub>l\<^sub>l M ((set xs', set ys'), to_remove) \<and>
+          vmtf_\<L>\<^sub>a\<^sub>l\<^sub>l \<A> M ((set xs', set ys'), to_remove) \<and>
           vmtf_ns_notin (ys' @ xs') m ns \<and>
-          (\<forall>L\<in>atms_of \<L>\<^sub>a\<^sub>l\<^sub>l. L < length ns) \<and>
-          (\<forall>L\<in>set (ys' @ xs'). L \<in> atms_of \<L>\<^sub>a\<^sub>l\<^sub>l)\<close>
+          (\<forall>L\<in>atms_of (\<L>\<^sub>a\<^sub>l\<^sub>l \<A>). L < length ns) \<and>
+          (\<forall>L\<in>set (ys' @ xs'). L \<in> atms_of (\<L>\<^sub>a\<^sub>l\<^sub>l \<A>))\<close>
     using atm_A by blast
 qed
 
 
-definition (in isasat_input_ops) vmtf_find_next_undef :: \<open>vmtf_remove_int \<Rightarrow> (nat, nat) ann_lits \<Rightarrow> (nat option) nres\<close> where
-\<open>vmtf_find_next_undef \<equiv> (\<lambda>((ns, m, fst_As, lst_As, next_search), to_remove) M. do {
-    WHILE\<^sub>T\<^bsup>\<lambda>next_search. ((ns, m, fst_As, lst_As, next_search), to_remove) \<in> vmtf M \<and>
-         (next_search \<noteq> None \<longrightarrow> Pos (the next_search) \<in># \<L>\<^sub>a\<^sub>l\<^sub>l)\<^esup>
+definition vmtf_find_next_undef :: \<open>nat multiset \<Rightarrow> vmtf_remove_int \<Rightarrow> (nat, nat) ann_lits \<Rightarrow> (nat option) nres\<close> where
+\<open>vmtf_find_next_undef \<A> = (\<lambda>((ns, m, fst_As, lst_As, next_search), to_remove) M. do {
+    WHILE\<^sub>T\<^bsup>\<lambda>next_search. ((ns, m, fst_As, lst_As, next_search), to_remove) \<in> vmtf \<A> M \<and>
+         (next_search \<noteq> None \<longrightarrow> Pos (the next_search) \<in># \<L>\<^sub>a\<^sub>l\<^sub>l \<A>)\<^esup>
       (\<lambda>next_search. next_search \<noteq> None \<and> defined_lit M (Pos (the next_search)))
       (\<lambda>next_search. do {
          ASSERT(next_search \<noteq> None);
          let n = the next_search;
-         ASSERT(Pos n \<in># \<L>\<^sub>a\<^sub>l\<^sub>l);
+         ASSERT(Pos n \<in># \<L>\<^sub>a\<^sub>l\<^sub>l  \<A>);
          ASSERT (n < length ns);
          RETURN (get_next (ns!n))
         }
@@ -1922,42 +1925,42 @@ definition (in isasat_input_ops) vmtf_find_next_undef :: \<open>vmtf_remove_int 
 
 lemma vmtf_find_next_undef_ref:
   assumes
-    vmtf: \<open>((ns, m, fst_As, lst_As, next_search), to_remove) \<in> vmtf M\<close>
-  shows \<open>vmtf_find_next_undef ((ns, m, fst_As, lst_As, next_search), to_remove) M
-     \<le> \<Down> Id (SPEC (\<lambda>L. ((ns, m, fst_As, lst_As, L), to_remove) \<in> vmtf M \<and>
-        (L = None \<longrightarrow> (\<forall>L\<in>#\<L>\<^sub>a\<^sub>l\<^sub>l. defined_lit M L)) \<and>
-        (L \<noteq> None \<longrightarrow> Pos (the L) \<in># \<L>\<^sub>a\<^sub>l\<^sub>l \<and> undefined_lit M (Pos (the L)))))\<close>
+    vmtf: \<open>((ns, m, fst_As, lst_As, next_search), to_remove) \<in> vmtf \<A> M\<close>
+  shows \<open>vmtf_find_next_undef \<A> ((ns, m, fst_As, lst_As, next_search), to_remove) M
+     \<le> \<Down> Id (SPEC (\<lambda>L. ((ns, m, fst_As, lst_As, L), to_remove) \<in> vmtf \<A> M \<and>
+        (L = None \<longrightarrow> (\<forall>L\<in>#\<L>\<^sub>a\<^sub>l\<^sub>l \<A>. defined_lit M L)) \<and>
+        (L \<noteq> None \<longrightarrow> Pos (the L) \<in># \<L>\<^sub>a\<^sub>l\<^sub>l \<A> \<and> undefined_lit M (Pos (the L)))))\<close>
 proof -
   obtain xs' ys' where
     vmtf_ns: \<open>vmtf_ns (ys' @ xs') m ns\<close> and
     fst_As: \<open>fst_As = hd (ys' @ xs')\<close> and
     lst_As: \<open>lst_As = last (ys' @ xs')\<close> and
     next_search: \<open>next_search = option_hd xs'\<close> and
-    abs_vmtf: \<open>vmtf_\<L>\<^sub>a\<^sub>l\<^sub>l M ((set xs', set ys'), to_remove)\<close> and
+    abs_vmtf: \<open>vmtf_\<L>\<^sub>a\<^sub>l\<^sub>l \<A> M ((set xs', set ys'), to_remove)\<close> and
     notin: \<open>vmtf_ns_notin (ys' @ xs') m ns\<close> and
-    atm_A: \<open>\<forall>L\<in>atms_of \<L>\<^sub>a\<^sub>l\<^sub>l. L < length ns\<close>
+    atm_A: \<open>\<forall>L\<in>atms_of (\<L>\<^sub>a\<^sub>l\<^sub>l \<A>). L < length ns\<close>
     using vmtf unfolding vmtf_def by fast
   have [simp]: \<open>index xs' (hd xs') = 0\<close> if \<open>xs' \<noteq> []\<close> for xs' :: \<open>'a list\<close>
     using that by (cases xs') auto
   have no_next_search_all_defined:
-    \<open>((ns', m', fst_As', lst_As', None), remove) \<in> vmtf M \<Longrightarrow>  x \<in># \<L>\<^sub>a\<^sub>l\<^sub>l \<Longrightarrow> defined_lit M x\<close>
+    \<open>((ns', m', fst_As', lst_As', None), remove) \<in> vmtf \<A> M \<Longrightarrow> x \<in># \<L>\<^sub>a\<^sub>l\<^sub>l \<A> \<Longrightarrow> defined_lit M x\<close>
     for x ns' m' fst_As' lst_As' remove
     by (auto simp: vmtf_def vmtf_\<L>\<^sub>a\<^sub>l\<^sub>l_def in_\<L>\<^sub>a\<^sub>l\<^sub>l_atm_of_in_atms_of_iff
         defined_lit_map lits_of_def)
   have next_search_\<L>\<^sub>a\<^sub>l\<^sub>l:
-    \<open>((ns', m', fst_As', lst_As', Some y), remove) \<in> vmtf M \<Longrightarrow> y \<in> atms_of \<L>\<^sub>a\<^sub>l\<^sub>l\<close>
+    \<open>((ns', m', fst_As', lst_As', Some y), remove) \<in> vmtf \<A> M \<Longrightarrow> y \<in> atms_of (\<L>\<^sub>a\<^sub>l\<^sub>l \<A>)\<close>
     for ns' m' fst_As' remove y lst_As'
     by (auto simp: vmtf_def vmtf_\<L>\<^sub>a\<^sub>l\<^sub>l_def in_\<L>\<^sub>a\<^sub>l\<^sub>l_atm_of_in_atms_of_iff
         defined_lit_map lits_of_def)
   have next_search_le_A':
-    \<open>((ns', m', fst_As', lst_As', Some y), remove) \<in> vmtf M \<Longrightarrow> y < length ns'\<close>
+    \<open>((ns', m', fst_As', lst_As', Some y), remove) \<in> vmtf \<A> M \<Longrightarrow> y < length ns'\<close>
     for ns' m' fst_As' remove y lst_As'
     by (auto simp: vmtf_def vmtf_\<L>\<^sub>a\<^sub>l\<^sub>l_def in_\<L>\<^sub>a\<^sub>l\<^sub>l_atm_of_in_atms_of_iff
         defined_lit_map lits_of_def)
   show ?thesis
     unfolding vmtf_find_next_undef_def
     apply (refine_vcg
-       WHILEIT_rule[where R=\<open>{(get_next (ns ! the a), a) |a. a \<noteq> None \<and> the a \<in> atms_of \<L>\<^sub>a\<^sub>l\<^sub>l}\<close>])
+       WHILEIT_rule[where R=\<open>{(get_next (ns ! the a), a) |a. a \<noteq> None \<and> the a \<in> atms_of (\<L>\<^sub>a\<^sub>l\<^sub>l \<A>)}\<close>])
     subgoal using vmtf by (rule wf_vmtf_get_next)
     subgoal using next_search vmtf by auto
     subgoal using vmtf by (auto dest!: next_search_\<L>\<^sub>a\<^sub>l\<^sub>l simp: image_image in_\<L>\<^sub>a\<^sub>l\<^sub>l_atm_of_in_atms_of_iff)
@@ -1977,27 +1980,29 @@ proof -
     done
 qed
 
-definition (in isasat_input_ops) vmtf_mark_to_rescore
+definition vmtf_mark_to_rescore
   :: \<open>nat \<Rightarrow> vmtf_remove_int \<Rightarrow> vmtf_remove_int\<close>
 where
   \<open>vmtf_mark_to_rescore L = (\<lambda>((ns, m, fst_As, next_search), to_remove).
      ((ns, m, fst_As, next_search), insert L to_remove))\<close>
 
 lemma vmtf_mark_to_rescore:
-  assumes L: \<open>L \<in>atms_of \<L>\<^sub>a\<^sub>l\<^sub>l\<close> and vmtf: \<open>((ns, m, fst_As, lst_As, next_search), to_remove) \<in> vmtf M\<close>
-  shows \<open>vmtf_mark_to_rescore L ((ns, m, fst_As, lst_As, next_search), to_remove) \<in> vmtf M\<close>
+  assumes
+    L: \<open>L \<in>atms_of (\<L>\<^sub>a\<^sub>l\<^sub>l \<A>)\<close> and
+    vmtf: \<open>((ns, m, fst_As, lst_As, next_search), to_remove) \<in> vmtf \<A> M\<close>
+  shows \<open>vmtf_mark_to_rescore L ((ns, m, fst_As, lst_As, next_search), to_remove) \<in> vmtf \<A> M\<close>
 proof -
   obtain xs' ys' where
     vmtf_ns: \<open>vmtf_ns (ys' @ xs') m ns\<close> and
     fst_As: \<open>fst_As = hd (ys' @ xs')\<close> and
     lst_As: \<open>lst_As = last (ys' @ xs')\<close> and
     next_search: \<open>next_search = option_hd xs'\<close> and
-    abs_vmtf: \<open>vmtf_\<L>\<^sub>a\<^sub>l\<^sub>l M ((set xs', set ys'), to_remove)\<close> and
+    abs_vmtf: \<open>vmtf_\<L>\<^sub>a\<^sub>l\<^sub>l \<A> M ((set xs', set ys'), to_remove)\<close> and
     notin: \<open>vmtf_ns_notin (ys' @ xs') m ns\<close> and
-    atm_A: \<open>\<forall>L\<in>atms_of \<L>\<^sub>a\<^sub>l\<^sub>l. L < length ns\<close> and
-    \<open>\<forall>L\<in>set (ys' @ xs'). L \<in> atms_of \<L>\<^sub>a\<^sub>l\<^sub>l\<close>
+    atm_A: \<open>\<forall>L\<in>atms_of (\<L>\<^sub>a\<^sub>l\<^sub>l \<A>). L < length ns\<close> and
+    \<open>\<forall>L\<in>set (ys' @ xs'). L \<in> atms_of (\<L>\<^sub>a\<^sub>l\<^sub>l \<A>)\<close>
     using vmtf unfolding vmtf_def by fast
-  moreover have \<open>vmtf_\<L>\<^sub>a\<^sub>l\<^sub>l M ((set xs', set ys'), insert L to_remove)\<close>
+  moreover have \<open>vmtf_\<L>\<^sub>a\<^sub>l\<^sub>l \<A> M ((set xs', set ys'), insert L to_remove)\<close>
     using abs_vmtf L unfolding vmtf_\<L>\<^sub>a\<^sub>l\<^sub>l_def
     by auto
   ultimately show ?thesis
@@ -2007,9 +2012,9 @@ qed
 lemma vmtf_unset_vmtf_tl:
   fixes M
   defines [simp]: \<open>L \<equiv> atm_of (lit_of (hd M))\<close>
-  assumes vmtf:\<open>((ns, m, fst_As, lst_As, next_search), remove) \<in> vmtf M\<close> and
-    L_N: \<open>L \<in> atms_of \<L>\<^sub>a\<^sub>l\<^sub>l\<close> and [simp]: \<open>M \<noteq> []\<close>
-  shows \<open>(vmtf_unset L ((ns, m, fst_As, lst_As, next_search), remove)) \<in> vmtf (tl M)\<close>
+  assumes vmtf:\<open>((ns, m, fst_As, lst_As, next_search), remove) \<in> vmtf \<A> M\<close> and
+    L_N: \<open>L \<in> atms_of (\<L>\<^sub>a\<^sub>l\<^sub>l \<A>)\<close> and [simp]: \<open>M \<noteq> []\<close>
+  shows \<open>(vmtf_unset L ((ns, m, fst_As, lst_As, next_search), remove)) \<in> vmtf \<A> (tl M)\<close>
      (is \<open>?S \<in> _\<close>)
 proof -
   obtain xs' ys' where
@@ -2017,10 +2022,10 @@ proof -
     fst_As: \<open>fst_As = hd (ys' @ xs')\<close> and
     lst_As: \<open>lst_As = last (ys' @ xs')\<close> and
     next_search: \<open>next_search = option_hd xs'\<close> and
-    abs_vmtf: \<open>vmtf_\<L>\<^sub>a\<^sub>l\<^sub>l M ((set xs', set ys'), remove)\<close> and
+    abs_vmtf: \<open>vmtf_\<L>\<^sub>a\<^sub>l\<^sub>l \<A> M ((set xs', set ys'), remove)\<close> and
     notin: \<open>vmtf_ns_notin (ys' @ xs') m ns\<close> and
-    atm_A: \<open>\<forall>L\<in>atms_of \<L>\<^sub>a\<^sub>l\<^sub>l. L < length ns\<close> and
-    ys'_xs'_\<L>\<^sub>a\<^sub>l\<^sub>l: \<open>\<forall>L\<in>set (ys' @ xs'). L \<in> atms_of \<L>\<^sub>a\<^sub>l\<^sub>l\<close>
+    atm_A: \<open>\<forall>L\<in>atms_of (\<L>\<^sub>a\<^sub>l\<^sub>l  \<A>). L < length ns\<close> and
+    ys'_xs'_\<L>\<^sub>a\<^sub>l\<^sub>l: \<open>\<forall>L\<in>set (ys' @ xs'). L \<in> atms_of (\<L>\<^sub>a\<^sub>l\<^sub>l \<A>)\<close>
     using vmtf unfolding vmtf_def by fast
   obtain ns' m' fst_As' next_search' remove'' lst_As' where
     S: \<open>?S = ((ns', m', fst_As', lst_As', next_search'), remove'')\<close>
@@ -2040,14 +2045,14 @@ proof -
        fst_As' = hd (ys' @ xs') \<and>
        lst_As' = last (ys' @ xs') \<and>
        next_search' = option_hd xs' \<and>
-       vmtf_\<L>\<^sub>a\<^sub>l\<^sub>l (tl M) ((set xs', set ys'), remove'') \<and>
-       vmtf_ns_notin (ys' @ xs') m' ns' \<and> (\<forall>L\<in>atms_of \<L>\<^sub>a\<^sub>l\<^sub>l. L < length ns') \<and>
-       (\<forall>L\<in>set (ys' @ xs'). L \<in> atms_of \<L>\<^sub>a\<^sub>l\<^sub>l)\<close>
+       vmtf_\<L>\<^sub>a\<^sub>l\<^sub>l \<A> (tl M) ((set xs', set ys'), remove'') \<and>
+       vmtf_ns_notin (ys' @ xs') m' ns' \<and> (\<forall>L\<in>atms_of (\<L>\<^sub>a\<^sub>l\<^sub>l \<A>). L < length ns') \<and>
+       (\<forall>L\<in>set (ys' @ xs'). L \<in> atms_of (\<L>\<^sub>a\<^sub>l\<^sub>l \<A>))\<close>
   proof (cases \<open>L \<in> set xs'\<close>)
     case True
     then have C[unfolded L_def]: \<open>\<not>(next_search = None \<or> stamp (ns ! the next_search) < stamp (ns ! L))\<close>
       by (subst L_ys'_iff[symmetric]) (use L_ys'_xs' in auto)
-    have abs_vmtf: \<open>vmtf_\<L>\<^sub>a\<^sub>l\<^sub>l (tl M) ((set xs', set ys'), remove)\<close>
+    have abs_vmtf: \<open>vmtf_\<L>\<^sub>a\<^sub>l\<^sub>l \<A> (tl M) ((set xs', set ys'), remove)\<close>
       using S abs_vmtf dist L_ys'_xs' True unfolding vmtf_\<L>\<^sub>a\<^sub>l\<^sub>l_def vmtf_unset_def
       by (cases M) (auto simp: C)
     show ?thesis
@@ -2091,16 +2096,16 @@ proof -
     moreover have \<open>next_search' = option_hd ?xs'\<close>
       by auto
     moreover {
-      have \<open>vmtf_\<L>\<^sub>a\<^sub>l\<^sub>l M ((set ?xs', set ?ys'), remove)\<close>
+      have \<open>vmtf_\<L>\<^sub>a\<^sub>l\<^sub>l \<A> M ((set ?xs', set ?ys'), remove)\<close>
         using abs_vmtf dist unfolding vmtf_\<L>\<^sub>a\<^sub>l\<^sub>l_def ys'_y_x
         by auto
-      then have \<open>vmtf_\<L>\<^sub>a\<^sub>l\<^sub>l (tl M) ((set ?xs', set ?ys'), remove)\<close>
+      then have \<open>vmtf_\<L>\<^sub>a\<^sub>l\<^sub>l \<A> (tl M) ((set ?xs', set ?ys'), remove)\<close>
         using dist L_y_ys unfolding vmtf_\<L>\<^sub>a\<^sub>l\<^sub>l_def ys'_y_x ys'_y_x
         by (cases M) auto
       }
     moreover have \<open>vmtf_ns_notin (?ys' @ ?xs') m ns\<close>
       using notin unfolding ys'_y_x by simp
-    moreover have \<open>\<forall>L\<in>set (?ys' @ ?xs'). L \<in> atms_of \<L>\<^sub>a\<^sub>l\<^sub>l\<close>
+    moreover have \<open>\<forall>L\<in>set (?ys' @ ?xs'). L \<in> atms_of (\<L>\<^sub>a\<^sub>l\<^sub>l \<A>)\<close>
       using ys'_xs'_\<L>\<^sub>a\<^sub>l\<^sub>l unfolding ys'_y_x by simp
     ultimately show ?thesis
       using S False atm_A unfolding vmtf_unset_def L_ys'_xs'[symmetric]
@@ -2111,12 +2116,12 @@ proof -
     by fast
 qed
 
-definition (in isasat_input_ops) vmtf_mark_to_rescore_and_unset :: \<open>nat \<Rightarrow> vmtf_remove_int \<Rightarrow> vmtf_remove_int\<close> where
+definition vmtf_mark_to_rescore_and_unset :: \<open>nat \<Rightarrow> vmtf_remove_int \<Rightarrow> vmtf_remove_int\<close> where
   \<open>vmtf_mark_to_rescore_and_unset L M = vmtf_mark_to_rescore L (vmtf_unset L M)\<close>
 
 lemma vmtf_append_remove_iff:
-  \<open>((ns, m, fst_As, lst_As, next_search), insert L b) \<in> vmtf M \<longleftrightarrow>
-     L \<in> atms_of \<L>\<^sub>a\<^sub>l\<^sub>l \<and> ((ns, m, fst_As, lst_As, next_search), b) \<in> vmtf M\<close>
+  \<open>((ns, m, fst_As, lst_As, next_search), insert L b) \<in> vmtf \<A> M \<longleftrightarrow>
+     L \<in> atms_of (\<L>\<^sub>a\<^sub>l\<^sub>l \<A>) \<and> ((ns, m, fst_As, lst_As, next_search), b) \<in> vmtf \<A> M\<close>
   (is \<open>?A \<longleftrightarrow> ?L \<and> ?B\<close>)
 proof
   assume vmtf: ?A
@@ -2125,20 +2130,20 @@ proof
     fst_As: \<open>fst_As = hd (ys' @ xs')\<close> and
     lst_As: \<open>lst_As = last (ys' @ xs')\<close> and
     next_search: \<open>next_search = option_hd xs'\<close> and
-    abs_vmtf: \<open>vmtf_\<L>\<^sub>a\<^sub>l\<^sub>l M ((set xs', set ys'), insert L b)\<close> and
+    abs_vmtf: \<open>vmtf_\<L>\<^sub>a\<^sub>l\<^sub>l \<A> M ((set xs', set ys'), insert L b)\<close> and
     notin: \<open>vmtf_ns_notin (ys' @ xs') m ns\<close> and
-    atm_A: \<open>\<forall>L\<in>atms_of \<L>\<^sub>a\<^sub>l\<^sub>l. L < length ns\<close> and
-    \<open>\<forall>L\<in>set (ys' @ xs'). L \<in> atms_of \<L>\<^sub>a\<^sub>l\<^sub>l\<close>
+    atm_A: \<open>\<forall>L\<in>atms_of (\<L>\<^sub>a\<^sub>l\<^sub>l \<A>). L < length ns\<close> and
+    \<open>\<forall>L\<in>set (ys' @ xs'). L \<in> atms_of (\<L>\<^sub>a\<^sub>l\<^sub>l \<A>)\<close>
     using vmtf unfolding vmtf_def by fast
-  moreover have \<open>vmtf_\<L>\<^sub>a\<^sub>l\<^sub>l M ((set xs', set ys'), b)\<close> and L: ?L
+  moreover have \<open>vmtf_\<L>\<^sub>a\<^sub>l\<^sub>l \<A> M ((set xs', set ys'), b)\<close> and L: ?L
     using abs_vmtf unfolding vmtf_\<L>\<^sub>a\<^sub>l\<^sub>l_def by auto
   ultimately have \<open>vmtf_ns (ys' @ xs') m ns \<and>
        fst_As = hd (ys' @ xs') \<and>
        next_search = option_hd xs' \<and>
        lst_As = last (ys' @ xs') \<and>
-       vmtf_\<L>\<^sub>a\<^sub>l\<^sub>l M ((set xs', set ys'), b) \<and>
-       vmtf_ns_notin (ys' @ xs') m ns \<and> (\<forall>L\<in>atms_of \<L>\<^sub>a\<^sub>l\<^sub>l. L < length ns) \<and>
-       (\<forall>L\<in>set (ys' @ xs'). L \<in> atms_of \<L>\<^sub>a\<^sub>l\<^sub>l)\<close>
+       vmtf_\<L>\<^sub>a\<^sub>l\<^sub>l \<A> M ((set xs', set ys'), b) \<and>
+       vmtf_ns_notin (ys' @ xs') m ns \<and> (\<forall>L\<in>atms_of (\<L>\<^sub>a\<^sub>l\<^sub>l \<A>). L < length ns) \<and>
+       (\<forall>L\<in>set (ys' @ xs'). L \<in> atms_of (\<L>\<^sub>a\<^sub>l\<^sub>l \<A>))\<close>
       by fast
   then show \<open>?L \<and> ?B\<close>
     using L unfolding vmtf_def by fast
@@ -2149,36 +2154,36 @@ next
     fst_As: \<open>fst_As = hd (ys' @ xs')\<close> and
     lst_As: \<open>lst_As = last (ys' @ xs')\<close> and
     next_search: \<open>next_search = option_hd xs'\<close> and
-    abs_vmtf: \<open>vmtf_\<L>\<^sub>a\<^sub>l\<^sub>l M ((set xs', set ys'), b)\<close> and
+    abs_vmtf: \<open>vmtf_\<L>\<^sub>a\<^sub>l\<^sub>l \<A> M ((set xs', set ys'), b)\<close> and
     notin: \<open>vmtf_ns_notin (ys' @ xs') m ns\<close> and
-    atm_A: \<open>\<forall>L\<in>atms_of \<L>\<^sub>a\<^sub>l\<^sub>l. L < length ns\<close> and
-    \<open>\<forall>L\<in>set (ys' @ xs'). L \<in> atms_of \<L>\<^sub>a\<^sub>l\<^sub>l\<close>
+    atm_A: \<open>\<forall>L\<in>atms_of (\<L>\<^sub>a\<^sub>l\<^sub>l \<A>). L < length ns\<close> and
+    \<open>\<forall>L\<in>set (ys' @ xs'). L \<in> atms_of (\<L>\<^sub>a\<^sub>l\<^sub>l \<A>)\<close>
     using vmtf unfolding vmtf_def by fast
-  moreover have \<open>vmtf_\<L>\<^sub>a\<^sub>l\<^sub>l M ((set xs', set ys'), insert L b)\<close>
+  moreover have \<open>vmtf_\<L>\<^sub>a\<^sub>l\<^sub>l \<A> M ((set xs', set ys'), insert L b)\<close>
     using vmtf abs_vmtf unfolding vmtf_\<L>\<^sub>a\<^sub>l\<^sub>l_def by auto
   ultimately have \<open>vmtf_ns (ys' @ xs') m ns \<and>
        fst_As = hd (ys' @ xs') \<and>
        next_search = option_hd xs' \<and>
        lst_As = last (ys' @ xs') \<and>
-       vmtf_\<L>\<^sub>a\<^sub>l\<^sub>l M ((set xs', set ys'), insert L b) \<and>
-       vmtf_ns_notin (ys' @ xs') m ns \<and> (\<forall>L\<in>atms_of \<L>\<^sub>a\<^sub>l\<^sub>l. L < length ns) \<and>
-       (\<forall>L\<in>set (ys' @ xs'). L \<in> atms_of \<L>\<^sub>a\<^sub>l\<^sub>l)\<close>
+       vmtf_\<L>\<^sub>a\<^sub>l\<^sub>l \<A> M ((set xs', set ys'), insert L b) \<and>
+       vmtf_ns_notin (ys' @ xs') m ns \<and> (\<forall>L\<in>atms_of (\<L>\<^sub>a\<^sub>l\<^sub>l \<A>). L < length ns) \<and>
+       (\<forall>L\<in>set (ys' @ xs'). L \<in> atms_of (\<L>\<^sub>a\<^sub>l\<^sub>l \<A>))\<close>
       by fast
-  then show \<open>?A\<close>
+  then show ?A
     unfolding vmtf_def by fast
 qed
 
 lemma vmtf_append_remove_iff':
-  \<open>(vm, insert L b) \<in> vmtf M \<longleftrightarrow>
-     L \<in> atms_of \<L>\<^sub>a\<^sub>l\<^sub>l \<and> (vm, b) \<in> vmtf M\<close>
+  \<open>(vm, insert L b) \<in> vmtf \<A> M \<longleftrightarrow>
+     L \<in> atms_of (\<L>\<^sub>a\<^sub>l\<^sub>l \<A>) \<and> (vm, b) \<in> vmtf \<A> M\<close>
   by (cases vm) (auto simp: vmtf_append_remove_iff)
 
 lemma vmtf_mark_to_rescore_unset:
   fixes M
   defines [simp]: \<open>L \<equiv> atm_of (lit_of (hd M))\<close>
-  assumes vmtf:\<open>((ns, m, fst_As, lst_As, next_search), remove) \<in> vmtf M\<close> and
-    L_N: \<open>L \<in> atms_of \<L>\<^sub>a\<^sub>l\<^sub>l\<close> and [simp]: \<open>M \<noteq> []\<close>
-  shows \<open>(vmtf_mark_to_rescore_and_unset L ((ns, m, fst_As, lst_As, next_search), remove)) \<in> vmtf (tl M)\<close>
+  assumes vmtf:\<open>((ns, m, fst_As, lst_As, next_search), remove) \<in> vmtf \<A> M\<close> and
+    L_N: \<open>L \<in> atms_of (\<L>\<^sub>a\<^sub>l\<^sub>l \<A>)\<close> and [simp]: \<open>M \<noteq> []\<close>
+  shows \<open>(vmtf_mark_to_rescore_and_unset L ((ns, m, fst_As, lst_As, next_search), remove)) \<in> vmtf \<A> (tl M)\<close>
      (is \<open>?S \<in> _\<close>)
   using vmtf_unset_vmtf_tl[OF assms(2-)[unfolded assms(1)]] L_N
   unfolding vmtf_mark_to_rescore_and_unset_def vmtf_mark_to_rescore_def
@@ -2187,7 +2192,7 @@ lemma vmtf_mark_to_rescore_unset:
 
 
 lemma vmtf_insert_sort_nth_code_preD:
-  assumes vmtf: \<open>vm \<in> vmtf M\<close>
+  assumes vmtf: \<open>vm \<in> vmtf \<A> M\<close>
   shows \<open>\<forall>x\<in>snd vm. x < length (fst (fst vm))\<close>
 proof -
   obtain ns m fst_As lst_As next_search remove where
@@ -2198,17 +2203,15 @@ proof -
     vmtf_ns: \<open>vmtf_ns (ys' @ xs') m ns\<close> and
     fst_As: \<open>fst_As = hd (ys' @ xs')\<close> and
     next_search: \<open>next_search = option_hd xs'\<close> and
-    abs_vmtf: \<open>vmtf_\<L>\<^sub>a\<^sub>l\<^sub>l M ((set xs', set ys'), remove)\<close> and
+    abs_vmtf: \<open>vmtf_\<L>\<^sub>a\<^sub>l\<^sub>l \<A> M ((set xs', set ys'), remove)\<close> and
     notin: \<open>vmtf_ns_notin (ys' @ xs') m ns\<close> and
-    atm_A: \<open>\<forall>L\<in>atms_of \<L>\<^sub>a\<^sub>l\<^sub>l. L < length ns\<close> and
-    \<open>\<forall>L\<in>set (ys' @ xs'). L \<in> atms_of \<L>\<^sub>a\<^sub>l\<^sub>l\<close>
+    atm_A: \<open>\<forall>L\<in>atms_of (\<L>\<^sub>a\<^sub>l\<^sub>l \<A>). L < length ns\<close> and
+    \<open>\<forall>L\<in>set (ys' @ xs'). L \<in> atms_of (\<L>\<^sub>a\<^sub>l\<^sub>l \<A>)\<close>
     using vmtf unfolding vmtf_def vm by fast
   show ?thesis
     using atm_A abs_vmtf unfolding vmtf_\<L>\<^sub>a\<^sub>l\<^sub>l_def
     by (auto simp: vm)
 qed
-
-end
 
 
 lemma vmtf_ns_Cons:
@@ -2296,9 +2299,9 @@ qed
 lemma length_vmtf_cons[simp]: \<open>length (vmtf_cons ns L n m) = length ns\<close>
   by (auto simp: vmtf_cons_def Let_def split: option.splits)
 
-lemma (in isasat_input_ops) wf_vmtf_get_prev:
-  assumes vmtf: \<open>((ns, m, fst_As, lst_As, next_search), to_remove) \<in> vmtf M\<close>
-  shows \<open>wf {(get_prev (ns ! the a), a) |a. a \<noteq> None \<and> the a \<in> atms_of \<L>\<^sub>a\<^sub>l\<^sub>l}\<close> (is \<open>wf ?R\<close>)
+lemma wf_vmtf_get_prev:
+  assumes vmtf: \<open>((ns, m, fst_As, lst_As, next_search), to_remove) \<in> vmtf \<A> M\<close>
+  shows \<open>wf {(get_prev (ns ! the a), a) |a. a \<noteq> None \<and> the a \<in> atms_of (\<L>\<^sub>a\<^sub>l\<^sub>l \<A>)}\<close> (is \<open>wf ?R\<close>)
 proof (rule ccontr)
   assume \<open>\<not> ?thesis\<close>
   then obtain f where
@@ -2310,9 +2313,9 @@ proof (rule ccontr)
     fst_As: \<open>fst_As = hd (ys' @ xs')\<close> and
     lst_As: \<open>lst_As = last (ys' @ xs')\<close> and
     next_search: \<open>next_search = option_hd xs'\<close> and
-    abs_vmtf: \<open>vmtf_\<L>\<^sub>a\<^sub>l\<^sub>l M ((set xs', set ys'), to_remove)\<close> and
+    abs_vmtf: \<open>vmtf_\<L>\<^sub>a\<^sub>l\<^sub>l \<A> M ((set xs', set ys'), to_remove)\<close> and
     notin: \<open>vmtf_ns_notin (ys' @ xs') m ns\<close> and
-    atm_A: \<open>\<forall>L\<in>atms_of \<L>\<^sub>a\<^sub>l\<^sub>l. L < length ns\<close>
+    atm_A: \<open>\<forall>L\<in>atms_of (\<L>\<^sub>a\<^sub>l\<^sub>l \<A>). L < length ns\<close>
     using vmtf unfolding vmtf_def by fast
   let ?f0 = \<open>the (f 0)\<close>
   have f_None: \<open>f i \<noteq> None\<close> for i
@@ -2376,7 +2379,7 @@ qed
 fun update_stamp where
   \<open>update_stamp xs n a = xs[a := VMTF_Node n (get_prev (xs!a)) (get_next (xs!a))]\<close>
 
-definition (in isasat_input_ops) vmtf_rescale :: \<open>vmtf \<Rightarrow> vmtf nres\<close> where
+definition vmtf_rescale :: \<open>vmtf \<Rightarrow> vmtf nres\<close> where
 \<open>vmtf_rescale = (\<lambda>(ns, m, fst_As, lst_As :: nat, next_search). do {
   (ns, m, _) \<leftarrow> WHILE\<^sub>T\<^bsup>\<lambda>_. True\<^esup>
      (\<lambda>(ns, n, lst_As). lst_As \<noteq>None)
@@ -2397,10 +2400,12 @@ lemma (in -) list_update_id':
   by auto
 (* End Move *)
 
-lemma (in isasat_input_bounded_nempty) vmtf_rescale_vmtf:
-  assumes vmtf: \<open>(vm, to_remove) \<in> vmtf M\<close>
+lemma vmtf_rescale_vmtf:
+  assumes vmtf: \<open>(vm, to_remove) \<in> vmtf \<A> M\<close> and
+    nempty: \<open>isasat_input_nempty \<A>\<close>and
+    bounded: \<open>isasat_input_bounded \<A>\<close>
   shows
-    \<open>vmtf_rescale vm \<le> SPEC (\<lambda>vm. (vm, to_remove) \<in> vmtf M \<and> fst (snd vm) \<le> uint32_max)\<close>
+    \<open>vmtf_rescale vm \<le> SPEC (\<lambda>vm. (vm, to_remove) \<in> vmtf \<A> M \<and> fst (snd vm) \<le> uint32_max)\<close>
     (is \<open>?A \<le> ?R\<close>)
 proof -
   obtain ns m fst_As lst_As next_search where
@@ -2412,18 +2417,18 @@ proof -
     fst_As: \<open>fst_As = hd (ys' @ xs')\<close> and
     lst_As: \<open>lst_As = last (ys' @ xs')\<close> and
     next_search: \<open>next_search = option_hd xs'\<close> and
-    abs_vmtf: \<open>vmtf_\<L>\<^sub>a\<^sub>l\<^sub>l M ((set xs', set ys'), to_remove)\<close> and
+    abs_vmtf: \<open>vmtf_\<L>\<^sub>a\<^sub>l\<^sub>l \<A> M ((set xs', set ys'), to_remove)\<close> and
     notin: \<open>vmtf_ns_notin (ys' @ xs') m ns\<close> and
-    atm_A: \<open>\<forall>L\<in>atms_of \<L>\<^sub>a\<^sub>l\<^sub>l. L < length ns\<close> and
-    in_lall: \<open>\<forall>L\<in>set (ys' @ xs'). L \<in> atms_of \<L>\<^sub>a\<^sub>l\<^sub>l\<close>
+    atm_A: \<open>\<forall>L\<in>atms_of (\<L>\<^sub>a\<^sub>l\<^sub>l \<A>). L < length ns\<close> and
+    in_lall: \<open>\<forall>L\<in>set (ys' @ xs'). L \<in> atms_of (\<L>\<^sub>a\<^sub>l\<^sub>l \<A>)\<close>
     using vmtf unfolding vmtf_def vm by fast
   have [dest]: \<open>ys' = [] \<Longrightarrow> xs' = [] \<Longrightarrow> False\<close> and
     [simp]: \<open>ys' = [] \<longrightarrow> xs' \<noteq> []\<close>
-    using abs_vmtf \<A>\<^sub>i\<^sub>n_nempty unfolding vmtf_\<L>\<^sub>a\<^sub>l\<^sub>l_def
+    using abs_vmtf nempty unfolding vmtf_\<L>\<^sub>a\<^sub>l\<^sub>l_def
     by (auto simp: atms_of_\<L>\<^sub>a\<^sub>l\<^sub>l_\<A>\<^sub>i\<^sub>n)
-  have 1: \<open>RES (vmtf M) = do {
+  have 1: \<open>RES (vmtf \<A> M) = do {
     a \<leftarrow> RETURN ();
-    RES (vmtf M)
+    RES (vmtf \<A> M)
     }\<close>
     by auto
   define zs where \<open>zs \<equiv> ys' @ xs'\<close>
@@ -2442,7 +2447,7 @@ proof -
     using vmtf lst_As unfolding I'_def vm zs_def[symmetric] by (auto simp: last_conv_nth)
 
 
-  have lits: \<open>literals_are_in_\<L>\<^sub>i\<^sub>n (Pos `# mset zs)\<close> and
+  have lits: \<open>literals_are_in_\<L>\<^sub>i\<^sub>n \<A> (Pos `# mset zs)\<close> and
     dist: \<open>distinct zs\<close>
     using abs_vmtf vmtf_ns_distinct[OF vmtf_ns] unfolding vmtf_def zs_def
       vmtf_\<L>\<^sub>a\<^sub>l\<^sub>l_def
@@ -2454,15 +2459,16 @@ proof -
     by (auto simp: tautology_decomp)
 
   have length_zs_le:  \<open>length zs < uint32_max\<close> using vmtf_ns_distinct[OF vmtf_ns]
-      using simple_clss_size_upper_div2[OF lits dist tauto]
+      using simple_clss_size_upper_div2[OF bounded lits dist tauto]
       by (auto simp: uint32_max_def)
 
-  have \<open>wf {(a, b). (a, b) \<in> {(get_prev (ns ! the a), a) |a. a \<noteq> None \<and> the a \<in> atms_of \<L>\<^sub>a\<^sub>l\<^sub>l}}\<close>
+  have \<open>wf {(a, b). (a, b) \<in> {(get_prev (ns ! the a), a) |a. a \<noteq> None \<and> the a \<in> atms_of (\<L>\<^sub>a\<^sub>l\<^sub>l \<A>)}}\<close>
     by (rule wf_subset[OF wf_vmtf_get_prev[OF vmtf[unfolded vm]]]) auto
   from wf_snd_wf_pair[OF wf_snd_wf_pair[OF this]]
-  have wf: \<open>wf {((_, _, a), (_, _, b)). (a, b) \<in> {(get_prev (ns ! the a), a) |a. a \<noteq> None \<and> the a \<in> atms_of \<L>\<^sub>a\<^sub>l\<^sub>l}}\<close>
+  have wf: \<open>wf {((_, _, a), (_, _, b)). (a, b) \<in> {(get_prev (ns ! the a), a) |a. a \<noteq> None \<and>
+      the a \<in> atms_of (\<L>\<^sub>a\<^sub>l\<^sub>l \<A>)}}\<close>
     by (rule wf_subset) auto
-  have zs_lall: \<open>zs ! (length zs - Suc n) \<in> atms_of \<L>\<^sub>a\<^sub>l\<^sub>l\<close> for n
+  have zs_lall: \<open>zs ! (length zs - Suc n) \<in> atms_of (\<L>\<^sub>a\<^sub>l\<^sub>l \<A>)\<close> for n
     using abs_vmtf nth_mem[of \<open>length zs - Suc n\<close> zs] unfolding zs_def vmtf_\<L>\<^sub>a\<^sub>l\<^sub>l_def
     by auto
   then have zs_le_ns[simp]: \<open>zs ! (length zs - Suc n) < length ns\<close> for n
@@ -2481,7 +2487,7 @@ proof -
                   \<in> {((_, _, a), _, _, b).
                     (a, b)
                     \<in> {(get_prev (ns ! the a), a) |a.
-                        a \<noteq> None \<and> the a \<in> atms_of \<L>\<^sub>a\<^sub>l\<^sub>l}})\<close>
+                        a \<noteq> None \<and> the a \<in> atms_of (\<L>\<^sub>a\<^sub>l\<^sub>l \<A>)}})\<close>
     if
       I': \<open>I' s'\<close> and
       cond: \<open>case s' of (ns, n, lst_As) \<Rightarrow> lst_As \<noteq> None\<close>
@@ -2617,7 +2623,7 @@ proof -
       using notin map_eq_nth_eq[OF eq_prev] map_eq_nth_eq[OF eq_next]
       unfolding zs_def[symmetric]
       by (auto simp: vmtf_ns_notin_def)
-    ultimately have \<open>((ns', n', fst_As, lst_As, next_search), to_remove) \<in> vmtf M\<close>
+    ultimately have \<open>((ns', n', fst_As, lst_As, next_search), to_remove) \<in> vmtf \<A> M\<close>
       using fst_As lst_As next_search abs_vmtf atm_A notin in_lall
       unfolding vmtf_def in_pair_collect_simp prod.case apply -
       apply (rule exI[of _ xs'])
@@ -2645,7 +2651,7 @@ proof -
   \<close>
   apply (rule WHILEIT_rule_stronger_inv_RES[where I' = I' and
       R = \<open>{((_, _, a), (_, _, b)). (a, b) \<in>
-         {(get_prev (ns ! the a), a) |a. a \<noteq> None \<and> the a \<in> atms_of \<L>\<^sub>a\<^sub>l\<^sub>l}}\<close>])
+         {(get_prev (ns ! the a), a) |a. a \<noteq> None \<and> the a \<in> atms_of (\<L>\<^sub>a\<^sub>l\<^sub>l \<A>)}}\<close>])
   subgoal
    by (rule wf)
   subgoal by fast
@@ -2663,16 +2669,13 @@ proof -
     done
 qed
 
+definition vmtf_flush
+   :: \<open>nat multiset \<Rightarrow> (nat,nat) ann_lits \<Rightarrow> vmtf_remove_int \<Rightarrow> vmtf_remove_int nres\<close>
+where
+  \<open>vmtf_flush \<A>\<^sub>i\<^sub>n = (\<lambda>M (vm, to_remove). RES (vmtf \<A>\<^sub>i\<^sub>n M))\<close>
 
-context isasat_input_bounded_nempty
-begin
-
-
-definition (in isasat_input_ops) vmtf_flush :: \<open>(nat,nat) ann_lits \<Rightarrow> vmtf_remove_int \<Rightarrow> vmtf_remove_int nres\<close> where
-\<open>vmtf_flush = (\<lambda>M (vm, to_remove). RES (vmtf M))\<close>
-
-definition (in isasat_input_bounded) vmtf_flush_int :: \<open>(nat,nat) ann_lits \<Rightarrow> _ \<Rightarrow> _ nres\<close> where
-\<open>vmtf_flush_int = (\<lambda>M (vm, (to_remove, h)). do {
+definition vmtf_flush_int :: \<open>nat multiset \<Rightarrow> (nat,nat) ann_lits \<Rightarrow> _ \<Rightarrow> _ nres\<close> where
+\<open>vmtf_flush_int \<A>\<^sub>i\<^sub>n = (\<lambda>M (vm, (to_remove, h)). do {
     ASSERT(\<forall>x\<in>set to_remove. x < length (fst vm));
     ASSERT(length to_remove \<le> uint32_max);
     to_remove' \<leftarrow> reorder_remove vm to_remove;
@@ -2681,7 +2684,7 @@ definition (in isasat_input_bounded) vmtf_flush_int :: \<open>(nat,nat) ann_lits
       then vmtf_rescale vm else RETURN vm);
     ASSERT(length to_remove' + fst (snd vm) \<le> uint64_max);
     (_, vm, h) \<leftarrow> WHILE\<^sub>T\<^bsup>\<lambda>(i, vm', h). i \<le> length to_remove' \<and> fst (snd vm') = i + fst (snd vm) \<and>
-          (i < length to_remove' \<longrightarrow> vmtf_en_dequeue_pre ((M, to_remove'!i), vm'))\<^esup>
+          (i < length to_remove' \<longrightarrow> vmtf_en_dequeue_pre \<A>\<^sub>i\<^sub>n ((M, to_remove'!i), vm'))\<^esup>
       (\<lambda>(i, vm, h). i < length to_remove')
       (\<lambda>(i, vm, h). do {
          ASSERT(i < length to_remove');
@@ -2693,16 +2696,16 @@ definition (in isasat_input_bounded) vmtf_flush_int :: \<open>(nat,nat) ann_lits
 
 lemma vmtf_change_to_remove_order:
   assumes
-    vmtf: \<open>((ns, m, fst_As, lst_As, next_search), to_remove) \<in> vmtf M\<close> and
+    vmtf: \<open>((ns, m, fst_As, lst_As, next_search), to_remove) \<in> vmtf \<A> M\<close> and
     CD_rem: \<open>((C, D), to_remove) \<in> distinct_atoms_rel\<close>
-  shows \<open>vmtf_flush_int M ((ns, m, fst_As, lst_As, next_search), (C, D))
-    \<le> \<Down> (Id \<times>\<^sub>r distinct_atoms_rel) (vmtf_flush M ((ns, m, fst_As, lst_As, next_search), to_remove))\<close>
+  shows \<open>vmtf_flush_int \<A> M ((ns, m, fst_As, lst_As, next_search), (C, D))
+    \<le> \<Down> (Id \<times>\<^sub>r distinct_atoms_rel) (vmtf_flush \<A> M ((ns, m, fst_As, lst_As, next_search), to_remove))\<close>
 proof -
   let ?vm = \<open>((ns, m, fst_As, lst_As, next_search), to_remove)\<close>
-  have vmtf_flush_alt_def: \<open>vmtf_flush M ?vm = do {
+  have vmtf_flush_alt_def: \<open>vmtf_flush \<A> M ?vm = do {
      _ \<leftarrow> RETURN ();
      _ \<leftarrow> RETURN ();
-     vm \<leftarrow> RES(vmtf M);
+     vm \<leftarrow> RES(vmtf \<A> M);
      RETURN (vm)
   }\<close>
     unfolding vmtf_flush_def by (auto simp: RES_RES_RETURN_RES RES_RETURN_RES vmtf)
@@ -2724,7 +2727,7 @@ proof -
       else RETURN x1)
       \<le> SPEC (\<lambda>c. (c, ()) \<in>
         {(vm ,vm'). uint64_max \<ge> length to_remove' + fst (snd vm) \<and>
-          (vm, D) \<in> vmtf M}) \<close>
+          (vm, D) \<in> vmtf \<A> M}) \<close>
     (is \<open>_ \<le> SPEC(\<lambda>c. (c, ()) \<in> ?rescale)\<close> is \<open>_ \<le> ?H\<close>)
   if
     \<open>x2 = (x1a, x2a)\<close> and
@@ -2737,7 +2740,7 @@ proof -
   proof -
     have \<open>vmtf_rescale x1 \<le> ?H\<close>
       apply (rule order_trans)
-      apply (rule vmtf_rescale_vmtf[of _ to_remove M])
+      apply (rule vmtf_rescale_vmtf[of _ to_remove \<A> M])
       subgoal using vmtf that by auto
       subgoal using that by (auto intro!: RES_refine simp: uint64_max_def uint32_max_def)
       done
@@ -2785,7 +2788,7 @@ proof -
       using that by (auto simp: )
     have D: \<open>D = to_remove\<close> and dist: \<open>distinct to_remove'\<close>
       using rel unfolding distinct_atoms_rel_def by auto
-    have in_lall: \<open>to_remove' ! x1 \<in> atms_of \<L>\<^sub>a\<^sub>l\<^sub>l\<close> if le': \<open>x1 < length to_remove'\<close> for x1
+    have in_lall: \<open>to_remove' ! x1 \<in> atms_of (\<L>\<^sub>a\<^sub>l\<^sub>l \<A>)\<close> if le': \<open>x1 < length to_remove'\<close> for x1
       using vmtf to_rem nth_mem[OF le'] by (auto simp: vmtf_def vmtf_\<L>\<^sub>a\<^sub>l\<^sub>l_def)
     have bound: \<open>fst (snd x1) + 1 \<le> uint64_max\<close> if \<open>0 < length to_remove'\<close>
         using rel vmtf to_rem that x1 by (cases to_remove') auto
@@ -2950,7 +2953,7 @@ context isasat_input_ops
 begin
 
 definition phase_saving :: \<open>phase_saver \<Rightarrow> bool\<close> where
-\<open>phase_saving \<phi> \<longleftrightarrow> (\<forall>L\<in>atms_of \<L>\<^sub>a\<^sub>l\<^sub>l. L < length \<phi>)\<close>
+\<open>phase_saving \<phi> \<longleftrightarrow> (\<forall>L\<in>atms_of (\<L>\<^sub>a\<^sub>l\<^sub>l \<A>). L < length \<phi>)\<close>
 
 text \<open>Save phase as given (e.g. for literals in the trail):\<close>
 definition save_phase :: \<open>nat literal \<Rightarrow> phase_saver \<Rightarrow> phase_saver\<close> where
